@base <https://purl.org/hmas/> .
@prefix : <> .
@prefix owl: <http://www.w3.org/2002/07/owl#> .
@prefix rdf: <http://www.w3.org/1999/02/22-rdf-syntax-ns#> .
@prefix xml: <http://www.w3.org/XML/1998/namespace> .
@prefix xsd: <http://www.w3.org/2001/XMLSchema#> .
@prefix rdfs: <http://www.w3.org/2000/01/rdf-schema#> .
@prefix cc: <http://creativecommons.org/ns#> .
@prefix vann: <http://purl.org/vocab/vann/> .
@prefix voaf: <http://purl.org/vocommons/voaf#> .
@prefix foaf: <http://xmlns.com/foaf/0.1/> .
@prefix schema: <http://schema.org/> .
@prefix dct: <http://purl.org/dc/terms/> .
@prefix skos: <http://www.w3.org/2004/02/skos/core#> .

#################################################################
#    Classes
#################################################################

:Organization a owl:Class ;
    rdfs:isDefinedBy :core ;
    rdfs:comment "An Organization is an entity situated on Agents and Artifacts, and regulated by a regulation system."@en ;
    rdfs:label "Organization"@en .

#################################################################
#    Properties
#################################################################

:isMemberOf a owl:ObjectProperty ;
    schema:domainIncludes :Agent ;
    schema:rangeIncludes :Organization ;
    rdfs:isDefinedBy :core ;
    rdfs:comment "A relation that refers to an Agent that belongs to an Organization."@en ;
    rdfs:label "is member of"@en .
      
:isMaterialOf a owl:ObjectProperty ;
    schema:domainIncludes :Artifact ;
    schema:rangeIncludes :Organization ;
    rdfs:isDefinedBy :core ;
    rdfs:comment "A relation that refers to an Artifact that belongs to an Organization."@en ;
    rdfs:label "is material of"@en .

:isSituatedOn a owl:ObjectProperty ;
    schema:domainIncludes :Organization ;
    schema:rangeIncludes :Agent, :Artifact ;
    rdfs:isDefinedBy :core ;
    rdfs:comment "A relation that refers to an Organization situated through its Members and Materials."@en ;
    rdfs:label "is situated on"@en .
