@base <https://purl.org/hmas/interaction> .
@prefix : <#> .
@prefix hmas: <https://purl.org/hmas/core#> .
@prefix owl: <http://www.w3.org/2002/07/owl#> .
@prefix rdfs: <http://www.w3.org/2000/01/rdf-schema#> .

#################################################################
#    Classes
#################################################################

###  https://purl.org/hmas/interaction#ActionExecution
:ActionExecution a owl:Class ;
                 rdfs:subClassOf :BehaviorExecution ;
                 rdfs:comment "A behavior execution that is the execution of exactly one context-free action, e.g. of a context-free HTTP request."@en ;
                 rdfs:label "action execution"@en .


###  https://purl.org/hmas/interaction#ActionSpecification
:ActionSpecification a owl:Class ;
                     rdfs:subClassOf :BehaviorSpecification ;
                     rdfs:comment "A specification that describes an action (e.g., through preconditions and postconditions) and how to execute the action, e.g. as a context-free request through a form."@en ;
                     rdfs:label "action specification"@en .


###  https://purl.org/hmas/interaction#BehaviorExecution
:BehaviorExecution a owl:Class ;
                   rdfs:comment "A course of action performed by an agent upon exploiting a behavior possibility."@en ;
                   rdfs:label "behavior execution"@en .


###  https://purl.org/hmas/interaction#BehaviorSpecification
:BehaviorSpecification a owl:Class ;
                       rdfs:comment "A specification that describes a behavior, for example, as procedural knowledge (e.g., AgentSpeak plan) or code-on-demand (e.g., a script that implements a behavior)."@en ;
                       rdfs:label "behavior specification"@en .


###  https://purl.org/hmas/interaction#Input
:Input a owl:Class ;
       rdfs:comment "An input of an action, which may include variables. The input may be used, for instance, in an action specification or in the representation of an action execution."@en ;
       rdfs:label "input"@en .

#################################################################
#    Properties
#################################################################

###  https://purl.org/hmas/interaction#expectsInput
:expectsInput a owl:ObjectProperty ;
              rdfs:domain :ActionSpecification ;
              rdfs:range :Input ;
              rdfs:comment "A relation between an action specification and the input that the specified action expects."@en ;
              rdfs:label "expects input"@en .


###  https://purl.org/hmas/interaction#hasForm
:hasForm a owl:ObjectProperty ;
         rdfs:domain :ActionSpecification ;
         rdfs:comment "A relation between an action specification and a form that describes how to execute the specified action."@en ;
         rdfs:label "has form"@en .


###  https://purl.org/hmas/interaction#hasSchema
:hasSchema a owl:ObjectProperty ;
           rdfs:comment "A relation between an input and the schema of the input."@en ;
           rdfs:label "has schema"@en .


###  https://purl.org/hmas/interaction#signifies
:signifies a owl:ObjectProperty ;
           rdfs:domain hmas:Signifier ;
           rdfs:range :BehaviorSpecification ;
           rdfs:comment "A relation between a signifier and a behavior specification it signifies."@en ;
           rdfs:label "signifies"@en .
