@base <https://purl.org/hmas/> .
@prefix : <> .
@prefix owl: <http://www.w3.org/2002/07/owl#> .
@prefix rdfs: <http://www.w3.org/2000/01/rdf-schema#> .

#################################################################
#    Classes
#################################################################

:ActionExecution a owl:Class ;
                 rdfs:isDefinedBy :interaction ;
                 rdfs:subClassOf :BehaviorExecution ;
                 rdfs:comment "A behavior execution that is the execution of exactly one context-free action, e.g. of a context-free HTTP request."@en ;
                 rdfs:label "action execution"@en,  "exécution de l'action"@fr .

:BehaviorExecution a owl:Class ;
                   rdfs:isDefinedBy :interaction ;
                   rdfs:comment "A course of action performed by an agent upon exploiting a behavior possibility."@en ;
                   rdfs:label "behavior execution"@en, "exécution du comportement"@fr .

:Input a owl:Class ;
       rdfs:isDefinedBy :interaction ;
       rdfs:comment "An input of an action, for example, in the representation of an action execution."@en ;
       rdfs:label "input"@en, "entrée"@fr .

#################################################################
#    Object Properties
#################################################################

:hasInput a owl:ObjectProperty ;
              rdfs:isDefinedBy :interaction ;
              rdfs:domain :ActionSpecification ;
              rdfs:range :Input ;
              rdfs:comment "A relation between an action execution and the input that it has."@en ;
              rdfs:label "has input"@en .

:signifies a owl:ObjectProperty ;
           rdfs:isDefinedBy :interaction ;
           rdfs:domain :Signifier ;
           rdfs:range :BehaviorSpecification ;
           rdfs:comment "A relation between a signifier and a behavior specification it signifies."@en ;
           rdfs:label "signifies"@en .
