@base <https://purl.org/hmas/regulation> .
@prefix : <#> .
@prefix hmas: <https://purl.org/hmas/core#> .
@prefix owl: <http://www.w3.org/2002/07/owl#> .
@prefix rdf: <http://www.w3.org/1999/02/22-rdf-syntax-ns#> .
@prefix rdfs: <http://www.w3.org/2000/01/rdf-schema#> .
@prefix schema: <http://schema.org/>.

#################################################################
#    Classes
#################################################################

:OrganizationSpecification a owl:Class ;
    rdfs:comment "An Organization Specification is a declarative specification used to enact one or multiple Organizations."@en ;
    rdfs:label "Organization Specification"@en .

:Organization a owl:Class ;
    rdfs:comment "An Organization is an entity situated on Agents and Artifacts, and regulated by a regulation system."@en ;
    rdfs:label "Organization"@en .

:OrganizationalGoal a owl:Class ;
    rdfs:comment "An Organizational Goal is an objective that outlines expected results and guide Organization members' efforts."@en ;
    rdfs:label "Organizational Goal"@en .

:OrganizationalValue a owl:Class ;
    rdfs:comment "An Organizational Value is a belief about socially or personally desirable end state or action that are explicitly or implicitly shared by members of an organization."@en ;
    rdfs:label "Organizational Value"@en .
        
:Role a owl:Class ;
    rdfs:comment "A Role is used to define the position that Agents can adopt in an Organization."@en ;
    rdfs:label "Role"@en .

:SocialRole a owl:Class ;
    rdfs:comment "A Social Role is used to define the position that Agents can adopt in an Organization in relation to a Group."@en ;
    rdfs:label "Social Role"@en .

:SpatialRole a owl:Class ;
    rdfs:comment "A Spatial Role is used to define the position that Agents can adopt in an Organization in relation to a Space."@en ;
    rdfs:label "Spatial Role"@en .

:Mission a owl:Class ;
    rdfs:comment "A Mission gathers Organizational Goals that can be achieved by Agents in an Organization in relation to a Social Activity."@en ;
    rdfs:label "Mission"@en .
    
:Facility a owl:Class ;
    rdfs:comment "A Facility is used to define functions that are offered by Materials in an Organization in relation to a Space."@en ;
    rdfs:label "Facility"@en .

#################################################################
#    Properties
#################################################################

:enacts a owl:ObjectProperty ;
    rdfs:domain :OrganizationSpecification ;
    rdfs:range :Organization ;
    rdfs:inverseOf :defines ;
    rdfs:comment "A relation that refers to an Organization that enacts an Organization Specification."@en ;
    rdfs:label "enacts"@en .
  
:defines a owl:ObjectProperty ;
    rdfs:domain :Organization ;
    rdfs:range :OrganizationSpecification ;
    owl:inverseOf :enacts ;
    rdfs:comment "A relation that refers to an Organization Specification that is enacted by an Organization."@en ;
    rdfs:label "defines"@en .

:hasGoal a owl:ObjectProperty ;
    rdfs:domain :Organization ;
    rdfs:range :OrganizationalGoal ;
    rdfs:comment "A relation that refers to an Organizational Goal of an Organization."@en ;
    rdfs:label "has goal"@en .

:hasValue a owl:ObjectProperty ;
    rdfs:domain :Organization ;
    rdfs:range :OrganizationalValue ;
    rdfs:comment "A relation that refers to an Organization Value of an Organization."@en ;
    rdfs:label "has value"@en .
      
:providesRole a owl:ObjectProperty ;
    rdfs:domain :Organization ;
    rdfs:range :Role ;
    rdfs:comment "A relation that refers to a Role made available to Agents in the context of an Organization."@en ;
    rdfs:label "provides role"@en .

:proposesMission a owl:ObjectProperty ;
    rdfs:domain :Organization ;
    rdfs:range :Mission ;
    rdfs:comment "A relation that refers to a Mission that can be executed in the context of an Organization."@en ;
    rdfs:label "proposes mission"@en .
    
:proposesFacility a owl:ObjectProperty ;
    rdfs:domain :Organization ;
    rdfs:range :Facility ;
    rdfs:comment "A relation that refers to a Facility that can be played in the context of an Organization."@en ;
    rdfs:label "proposes facility"@en .
    
:isSituatedOn a owl:ObjectProperty ;
    schema:domainIncludes :Organization ;
    schema:rangeIncludes :Agent, :Artifact ;
    rdfs:comment "An Organization is situated on Agents and Artifacts."@en ;
    rdfs:label "is situated on"@en .

:isMemberOf a owl:ObjectProperty ;
    rdfs:domain :Agent ;
    rdfs:range :Organization ;
    rdfs:comment "A Member refers to an Agent that belongs to an Organization."@en ;
    rdfs:label "is member of"@en .

:isMaterialOf a owl:ObjectProperty ;
    rdfs:domain :Artifact ;
    rdfs:range :Organization ;
    rdfs:comment "A Material refers to an Artifact that belongs to an Organization."@en ;
    rdfs:label "is material of"@en .
