@base <https://purl.org/hmas/regulation> .
@prefix : <#> .
@prefix hmas: <https://purl.org/hmas/core#> .
@prefix owl: <http://www.w3.org/2002/07/owl#> .
@prefix rdf: <http://www.w3.org/1999/02/22-rdf-syntax-ns#> .
@prefix rdfs: <http://www.w3.org/2000/01/rdf-schema#> .
@prefix schema: <http://schema.org/> .

#################################################################
#    Classes
#################################################################

:SocialRole a owl:Class ;
    rdfs:comment "A Social Role is used to define the position that Agents can adopt in an Organization in relation to a Group."@en ;
    rdfs:label "Social Role"@en .
    
:Group a owl:Class ;
    rdfs:comment "A Group is a set of Agents that can exist in the structure of an Organization."@en ;
    rdfs:label "Group"@en .
    
#################################################################
#    Properties
#################################################################

:structures a owl:ObjectProperty ;
    schema:domainIncludes :Group ;
    schema:rangeIncludes :Organization ;
    rdfs:inverseOf :isStructuredBy ;
    rdfs:comment "A relation that refers to a Group that structures an Organization."@en ;
    rdfs:label "structures"@en .

:isStructuredBy a owl:ObjectProperty ;
    schema:domainIncludes :Organization ;
    schema:rangeIncludes :Group ;
    rdfs:inverseOf :structures ;
    rdfs:comment "A relation that refers to an Organization that is structured by a Group."@en ;
    rdfs:label "is structured by"@en .
    
:plays a owl:ObjectProperty ;
    schema:domainIncludes hmas:Agent ;
    schema:rangeIncludes :SocialRole ;
    rdfs:comment "A relation that refers to a Social Role that an Agent plays in the context of an Organization."@en ;
    rdfs:label "plays"@en .

:belongsTo a owl:ObjectProperty ;
    schema:domainIncludes :SocialRole ;
    schema:rangeIncludes :Group ;
    rdfs:comment "A relation that refers to a Social Role that is part of a Group."@en ;
    rdfs:label "belongs to"@en .

:isLinkedTo a owl:ObjectProperty ;
    schema:domainIncludes :SocialRole ;
    schema:rangeIncludes :SocialRole ;
    rdfs:comment "A relation that refers to a relation between Social Roles."@en ;
    rdfs:label "is linked to"@en .
    
:relatesTo a owl:ObjectProperty ;
    schema:domainIncludes :Group ;
    schema:rangeIncludes :Group ;
    rdfs:comment "A relation that refers to a relation between Groups."@en ;
    rdfs:label "relates to"@en .
