@prefix hmas: <https://purl.org/hmas/> .
@prefix owl: <http://www.w3.org/2002/07/owl#> .
@prefix rdfs: <http://www.w3.org/2000/01/rdf-schema#> .
@prefix schema: <http://schema.org/> .

#################################################################
#    Classes
#################################################################

hmas:Role a owl:Class ;
    rdfs:comment "A Role defines the position that Agents can adopt in an Organization."@en ;
    rdfs:label "Role"@en .

hmas:Group a owl:Class ;
    rdfs:comment "A Group is a set of Agents that can exist in the structure of an Organization."@en ;
    rdfs:label "Group"@en .
    
#################################################################
#    Properties
#################################################################

hmas:structures a owl:ObjectProperty ;
    schema:domainIncludes hmas:Group ;
    schema:rangeIncludes hmas:Organization ;
    rdfs:inverseOf hmas:isStructuredBy ;
    rdfs:comment "A relation that refers to a Group that structures an Organization."@en ;
    rdfs:label "structures"@en .

hmas:isStructuredBy a owl:ObjectProperty ;
    schema:domainIncludes hmas:Organization ;
    schema:rangeIncludes hmas:Group ;
    rdfs:inverseOf hmas:structures ;
    rdfs:comment "A relation that refers to an Organization that is structured by a Group."@en ;
    rdfs:label "is structured by"@en .
    
hmas:plays a owl:ObjectProperty ;
    schema:domainIncludes hmas:Agent ;
    schema:rangeIncludes hmas:Role ;
    rdfs:comment "A relation that refers to a Role that an Agent plays in the context of an Organization."@en ;
    rdfs:label "plays"@en .

hmas:belongsTo a owl:ObjectProperty ;
    schema:domainIncludes hmas:Role ;
    schema:rangeIncludes hmas:Group ;
    rdfs:comment "A relation that refers to a Role that is part of a Group."@en ;
    rdfs:label "belongs to"@en .

hmas:isLinkedTo a owl:ObjectProperty ;
    schema:domainIncludes hmas:Role ;
    schema:rangeIncludes hmas:Role ;
    rdfs:comment "A relation that refers to an interaction relation between two Roles."@en ;
    rdfs:label "is linked to"@en .
    
hmas:isSubGroupOf a owl:ObjectProperty ;
    schema:domainIncludes hmas:Group ;
    schema:rangeIncludes hmas:Group ;
    rdfs:comment "A relation that refers to a subgroup relation between two Groups."@en ;
    rdfs:label "is subgroup of"@en .
