@base <https://purl.org/hmas/core> .
@prefix : <#> .
@prefix owl: <http://www.w3.org/2002/07/owl#> .
@prefix rdfs: <http://www.w3.org/2000/01/rdf-schema#> .
@prefix skos: <http://www.w3.org/2004/02/skos/core#>.
@prefix dct: <http://purl.org/dc/terms/>.


#################################################################
#    Classes
#################################################################

:Hostable a owl:Class ;
        rdfs:comment "A resource that can be hosted on a MAS platform"@en ;
        skos:example "an agent, an artefact, other MAS platforms, workspaces, resource profiles, signifiers, organizations, can be hosted on a MAS platform"@en ;
        rdfs:label "Hostable"@en, "Hébergeable"@fr ;
        rdfs:seeAlso <https://github.com/HyperAgents/ns.hyperagents.org/issues/8> ;
        rdfs:seeAlso <https://github.com/HyperAgents/ns.hyperagents.org/issues/23> .

:Agent a owl:Class ;
        rdfs:comment "An entity that is capable of autonomous behavior."@en ;
        rdfs:label "Agent"@en, "Agent"@fr ;
        rdfs:subClassOf :Hostable .

:ResourceProfile a owl:Class ;
        rdfs:comment "Structured data describing a resource through general metadata, domain- and application-specific metadata, and signifiers."@en ;
        skos:example "e.g., a Thing Description document, a Hydra document, an Socio-Technical Network platform description, a fipa:AgentDescription"@en ;
        rdfs:label "Resource Profile"@en, "Profil de Ressource"@fr .

:HypermediaMASPlatform a owl:Class ;
        rdfs:comment "A Hypermedia MAS platform is a system providing a collection of features to support Hypermedia MAS. Common features include support for communication and interaction, runtime environments for agents, artifacts, or organizations, etc."@en ;
        rdfs:label "MAS Platform"@en, "Platforme SMA"@fr ;
        skos:example "Examples of hmas:HypermediaMASPlatform include Twitter, Facebook, a JADE node/delpoyment, or a JaCaMo node/delpoyment — all of which provide features that could support Hypermedia MAS & hybrid communities."@en .

:Signifier a owl:Class ;
         rdfs:label "Signifier"@en, "Signifiant"@fr  ;
         rdfs:comment "A perceivable sign/cue that can be interpreted meaningfully by an agent to reveal information about a behavior possibility."@en .

#################################################################
#    Object Properties
#################################################################

:hasProfile a owl:ObjectProperty, owl:AsymmetricProperty ;
            rdfs:range :ResourceProfile ;
            owl:inverseOf :isProfileOf ;
            rdfs:comment "A relation that links a resource to its profile."@en ;
            rdfs:label "has profile"@en .

:isProfileOf a owl:ObjectProperty ;
           owl:inverseOf :hasProfile ;
           rdfs:domain :ResourceProfile ;
           rdfs:comment "A relation that links a resource profile to the resource it is a profile of."@en ;
           skos:example ""@en ;
           rdfs:label "is profile of"@en .

:exposesSignifier a owl:ObjectProperty ;
            rdfs:domain :ResourceProfile ;
            rdfs:range :Signifier ;
            rdfs:comment "A relation between a resource profile and a signifier it exposes."@en ; 
            rdfs:label "exposes signifier"@en .

:isExposedIn a owl:ObjectProperty ;
            rdfs:label "is exposed in"@en ;
            owl:inverseOf :exposesSignifier ;
            rdfs:comment "A relation between a signifier and a resource profile it is exposed in."@en ;
            rdfs:domain :Signifier ;
            rdfs:range :ResourceProfile .

:hosts a owl:ObjectProperty, owl:AsymmetricProperty ;
            rdfs:domain :HypermediaMASPlatform ;
            rdfs:range :Hostable ;
            rdfs:comment "A relation that refers to an information resource or a process (e.g., agent) that is hosted on a platform. A hosting relation might have further implications, e.g. the usage of the hosted resource (or the usage of platform resources by the hosted resource) could be subject to terms of service or data licensing policies specific to the hosting platform."@en ;
            rdfs:label "hosts"@en ;
            dct:source <https://github.com/HyperAgents/ns.hyperagents.org/issues/8#issuecomment-1025991719> ;
            rdfs:seeAlso <https://github.com/HyperAgents/ns.hyperagents.org/issues/18> ;
            rdfs:seeAlso <https://github.com/HyperAgents/ns.hyperagents.org/issues/49> .

:isHostedOn a owl:ObjectProperty, owl:AsymmetricProperty ; 
            owl:inverseOf :hosts ;
            rdfs:domain :Hostable ;
            rdfs:range :HypermediaMASPlatform ;
            rdfs:comment "A relations that refers to the platform that hosts the resource. "@en ;
            rdfs:label "is hosted on"@en .