@base <https://ci.mines-stetienne.fr/regulation> .
@prefix : <#> .
@prefix owl: <http://www.w3.org/2002/07/owl#> .
@prefix hmas: <https://ci.mines-stetienne.fr/hmas> .
@prefix hreg: <https://ci.mines-stetienne.fr/regulation> .
@prefix rdf: <http://www.w3.org/1999/02/22-rdf-syntax-ns#> .
@prefix xml: <http://www.w3.org/XML/1998/namespace> .
@prefix xsd: <http://www.w3.org/2001/XMLSchema#> .
@prefix rdfs: <http://www.w3.org/2000/01/rdf-schema#> .
@prefix time: <http://www.w3.org/2006/time#> .

<#> rdf:type owl:Ontology ;
                                       owl:imports <https://ci.mines-stetienne.fr/hmas#> .



:RegulativeNorm rdf:type owl:Class ;
           rdfs:comment "A specification of the standard behaviors one expects from others in an organization."@en ;
           rdfs:label "Norm"@en .

:PossibleWorld rdf:type owl:Class ;
  rdfs:comment "A possible world is a ressource that describes a state of affair of the world."@en ;
  rdfs:label "Normative Context"@en .


#:Modality rdf:subClassOf :PossibleWorld ;
#  rdfs:comment "A modality specifies qualities of the truth contained in a possible world."@en ;
#  rdfs:label "Normative Context"@en .

:NormativeContext rdf:subClassOf :PossibleWorld ;
  rdfs:comment "A context in which a norm is applicable."@en ;
  rdfs:label "Normative Context"@en .

:Obligation rdf:subClassOf :PossibleWorld ;
  rdfs:comment "A possible world that describes an obligation."@en ;
  rdfs:label "Obligation"@en .

:Permission rdf:subClassOf :PossibleWorld ;
  rdfs:comment "A possible world that describes a permission."@en ;
  rdfs:label "Permission"@en .

:Prohibition rdf:subClassOf :PossibleWorld ;
  rdfs:comment "A possible world that describes a prohibition."@en ;
  rdfs:label "Prohibition"@en .

#:AuthorityRole rdf:subClassOf hreg:SocialRole ;
#           rdfs:comment "The authority who has a power to apply a norm and which is in charge of applying the norm. It may be an :Agent or an :Organization. "@en ;
#           rdfs:label "Authority"@en .

#:enforcesNorm rdf:type owl:ObjectProperty ;
#		rdfs:domain hreg:Organization ;
#                rdfs:range :RegulativeNorm ;
#                rdfs:comment "An organization enforces a norm. "@en ;
#                rdfs:label "enforces the norm"@en .        

#:definesNorm rdf:type owl:ObjectProperty ;
#		rdfs:domain hreg:OrganizationSpecification ;
#                rdfs:range :RegulativeNorm ;
#                rdfs:comment "An organization Specification defines a norm. "@en ;
#                rdfs:label "defines the norm"@en .        

#:hasNormativeTarget rdf:type owl:ObjectProperty ;
#		rdfs:domain :RegulativeNorm ;
#		rdfs:range :Role ;
#		rdfs:comment "An agent or a group of agents concerned by a norm." ;
#		rdfs:label "has normative target".

#:hasNormativeObject rdf:type owl:ObjectProperty ;
#		rdfs:domain :RegulativeNorm ;
#		rdfs:range :Behavior ;
#		rdfs:comment "A specification which defines the expected behavior by describing explicitly the expected behavior or implictly by describing the state of affairs.";
#		rdfs:label "has normative object".
	  
#:hasPowerOn rdf:type owl:ObjectProperty ;
#		rdfs:domain :Norm ;
#                rdfs:range :AuthorityRole;
#                rdfs:comment "It defines who is the authority in charge of applying the norm. "@en ;
#                rdfs:label "has normative requirement"@en .


:hasDeonticSpecification rdf:type owl:ObjectProperty ;
                rdfs:domain :PossibleWorld ;
                rdfs:range :RegulativeNorm ;
                rdfs:comment "A possible world may have some deontic specifications. "@en ;
                rdfs:label "has deontic specification"@en .

:prohibits rdf:type owl:ObjectProperty ;
                rdfs:domain :RegulativeNorm ;
                rdfs:range :Prohibition ;
                rdfs:comment "A prohibition is associated with a norm and describes a state of affairs that shouldn't be verified when a norm is applied. "@en ;
                rdfs:label "prohibits"@en .

:permits rdf:type owl:ObjectProperty ;
                rdfs:domains :RegulativeNorm ;
                rdfs:range :Permission ;
                rdfs:comment "A permission is associated with a norm and describes a state of affairs which is explicitly permitted when a norm is applied."@en ;
                rdfs:label "allows"@en .

:obliges rdf:type owl:ObjectProperty ;
		rdfs:domain :RegulativeNorm ;
                rdfs:range :Obligation ;
                rdfs:comment "An obligation is associated with a norm and describes a state of affairs that must be maintained when a norm is applied."@en ;
                rdfs:label "obliges"@en .



#:hasException rdf:type owl:ObjectProperty ;
#               rdfs:domain :Contextable .
#               rdfs:comment "Associates exceptions to a context of application of a norm"@en ;
#               rdfs:label "has exception"@en .
  

:hasNormativeContext rdf:type owl:ObjectProperty ;
  rdfs:domain :RegulativeNorm ;
  rdfs:range :NormativeContext ;
  #rdfs:range rdfs:Container ;
  rdfs:range :NormativeContext ;
  rdfs:comment "A specification which defines when a norm is applicable. "@en ;
  rdfs:label "has normative context"@en .


:hasRespectStatus rdf:type owl:ObjectProperty ;
  rdfs:domain :RegulativeNorm ;
  rdfs:range xsd:boolean ;
  rdfs:comment "Indicates whether a norm has been respected or not"@en ;
  rdfs:label "has respect status"@en .









