@base <https://purl.org/hmas/> .
@prefix : <> .
@prefix owl: <http://www.w3.org/2002/07/owl#> .
@prefix rdf: <http://www.w3.org/1999/02/22-rdf-syntax-ns#> .
@prefix xml: <http://www.w3.org/XML/1998/namespace> .
@prefix xsd: <http://www.w3.org/2001/XMLSchema#> .
@prefix rdfs: <http://www.w3.org/2000/01/rdf-schema#> .
@prefix cc: <http://creativecommons.org/ns#> .
@prefix vann: <http://purl.org/vocab/vann/> .
@prefix voaf: <http://purl.org/vocommons/voaf#> .
@prefix foaf: <http://xmlns.com/foaf/0.1/> .
@prefix schema: <http://schema.org/> .
@prefix dct: <http://purl.org/dc/terms/> .
@prefix skos: <http://www.w3.org/2004/02/skos/core#> .

#################################################################
#    Classes
#################################################################

:ProcessScheme a owl:Class ;
    rdfs:isDefinedBy :regulation ;
    rdfs:comment "A Process Scheme is an entity that represents a set of connected Activity Schemes."@en ;
    rdfs:label "process scheme"@en, "schéma de processus"@fr .
    
:ActivityScheme a owl:Class ;
    rdfs:isDefinedBy :regulation ;
    rdfs:comment "An Activity Scheme is a plan for an activity intended to achieve an Organizational Goal."@en ;
    rdfs:label "activity scheme"@en, "schéma d'activité"@fr ;
    skos:note "The concept of activity can be the execution of a simple action, a complex set of actions, or any other useful arrangement employed to achieving organizational goals. An activity can be represented using, for instance, the PROV Ontology (https://www.w3.org/TR/prov-o/)."@en .

:Mission a owl:Class ;
    rdfs:isDefinedBy :regulation ;
    rdfs:comment "A Mission gathers the Organizational Goals that Agents have to achieve in the context of a Process Scheme."@en ;
    rdfs:label "mission"@en, "mission"@fr .
    
#################################################################
#    Properties
#################################################################

:isMissionOf a owl:ObjectProperty ;
    rdfs:isDefinedBy :regulation ;
    rdfs:domain :Mission ;
    rdfs:range :Agent ;
    rdfs:comment "A relation that refers to an Agent involved in a Mission."@en ;
    rdfs:label "is mission of"@en, "est la mission de"@fr .

:isMissionFor a owl:ObjectProperty ;
    rdfs:isDefinedBy :regulation ;
    rdfs:domain :Mission ;
    rdfs:range :OrganizationalGoal ;
    rdfs:comment "A relation that refers to an Organizational Goal involved in a Mission."@en ;
    rdfs:label "is mission for"@en, "est la mission pour"@fr .

:isMissionIn a owl:ObjectProperty ;
    rdfs:isDefinedBy :regulation ;
    rdfs:domain :Mission ;
    rdfs:range :ProcessScheme ;
    rdfs:comment "A relation that refers to a Process Scheme involved in a Mission."@en ;
    rdfs:label "is mission in"@en, "est la mission en"@fr .

:hasMissionRelationshipWith a owl:ObjectProperty ;
    rdfs:isDefinedBy :regulation ;
    rdfs:domain :Mission ;
    rdfs:range :Mission ;
    rdfs:comment "A relation that refers to the relationship between two Missions, e.g., complementary missions."@en ;
    rdfs:label "has mission relationship with"@en, "a une relation de mission avec"@fr .
    
:isSubOrganizationalGoalOf a owl:ObjectProperty ;
    rdfs:isDefinedBy :regulation ;
    rdfs:domain :OrganizationalGoal ;
    rdfs:range :OrganizationalGoal ;
    rdfs:comment "A relation that refers to a hierarchical relationship between two Organizational Goals. A Sub-Organizational Goal is an Organizational Goal that has to be achieved for the parent Organizational Goal to be achieved."@en ;
    rdfs:label "is sub-organizational goal of"@en, "est le but sous-organisationnel de"@fr .
    
:achievesOrganizationalGoal a owl:ObjectProperty ;
    rdfs:isDefinedBy :regulation ;
    rdfs:domain :ActivityScheme ;
    rdfs:range :OrganizationalGoal ;
    rdfs:comment "A relation that refers to an Organizational Goal coordinated by an Activity Scheme."@en ;
    rdfs:label "achieves organizational goal"@en, "coordonner but organisationnel"@fr .

:proposesProcessScheme a owl:ObjectProperty ;
    rdfs:isDefinedBy :regulation ;
    rdfs:domain :Organization ;
    rdfs:range :ProcessScheme ;
    rdfs:comment "A relation that refers to a Process Scheme that can be carried out within an Organization."@en ;
    rdfs:label "proposes activity scheme"@en, "propose une schéma d'activité"@fr .

:hasRootActivityScheme a owl:ObjectProperty ;
    rdfs:isDefinedBy :regulation ;
    rdfs:domain :ProcessScheme ;
    rdfs:range :RootActivityScheme ;
    rdfs:comment "A relation that refers to the Root Activity Scheme (i.e., an Activity Scheme origin of a set of connected Activity Schemes) associated to a Process Scheme."@en ;
    rdfs:label "has root activity scheme"@en, "a un schéma d'activité racine"@fr .
    
:proposesActivityScheme a owl:ObjectProperty ;
    rdfs:isDefinedBy :regulation ;
    rdfs:domain :Organization ;
    rdfs:range :ActivityScheme ;
    rdfs:comment "A relation that refers to an Activity Scheme that can be carried out within an Organization."@en ;
    rdfs:label "proposes activity scheme"@en, "propose une schéma d'activité"@fr .
    
:isDependentOnActivityScheme a owl:ObjectProperty ;
    rdfs:isDefinedBy :regulation ;
    rdfs:domain :ActivityScheme ;
    rdfs:range :ActivityScheme ;
    rdfs:comment "A relation that refers to the way in which two Activity Schemes are related to each other, and one is affected by the other."@en ;
    rdfs:label "is dependent on activity scheme"@en, "dépend du schéma d'activité"@fr .
