@base <https://purl.org/hmas/> .
@prefix : <> .
@prefix owl: <http://www.w3.org/2002/07/owl#> .
@prefix rdfs: <http://www.w3.org/2000/01/rdf-schema#> .
@prefix skos: <http://www.w3.org/2004/02/skos/core#> .
@prefix dcterms: <http://purl.org/dc/terms/> .

:Affordance a skos:Concept ;
    rdfs:isDefinedBy :core ;
    skos:prefLabel "affordance"@en ;
    skos:definition "A behavior possibility that is a relationship between an ability of an agent and a situation that includes agents and features of the environment."@en ;
    skos:scopeNote "The definition of the concept follows affordance theorists [Chemero and Turvey, 2007] and is provided to support the discussion, management, and modelling of signifiers, which reveal information about affordances [Norman, 2013]. For example, the association between the two terms enables examining the dynamic exposure of signifiers based on the run-time availability of agent abilities and situations, or the modelling of signifiers that reveal information about affordances for both artificial and human agents."@en ;
    dcterms:references _:chemeroTurvey2007 ;
    dcterms:references _:norman2013 .

_:chemeroTurvey2007 dcterms:bibliographicCitation "Chemero, A., & Turvey, M. T. (2007). Complexity, hypersets, and the ecological perspective on perception-action. Biological Theory, 2(1), 23-36."@en ;
    rdfs:label "Chemero and Turvey, 2007"@en .

_:norman2013 dcterms:bibliographicCitation "Norman, D. (2013). The design of everyday things: Revised and expanded edition. Basic books."@en ;
    rdfs:label "Norman, 2013"@en .

#################################################################
#    Classes
#################################################################

:Signifier a owl:Class ;
         rdfs:isDefinedBy :core ;
         rdfs:label "Signifier"@en, "Signifiant"@fr  ;
         rdfs:comment "A perceivable sign/cue that can be interpreted meaningfully by an agent to reveal information about a behavior possibility."@en ;
         rdfs:subClassOf :Hostable .

#################################################################
#    Properties
#################################################################

:isExposedIn a owl:ObjectProperty ;
            rdfs:isDefinedBy :core ;
            rdfs:label "is exposed in"@en ;
            owl:inverseOf :exposesSignifier ;
            rdfs:comment "A relation between a signifier and a resource profile it is exposed in."@en ;
            rdfs:domain :Signifier ;
            rdfs:range :ResourceProfile .
