@base <https://ci.mines-stetienne.fr/hmas> .
@prefix : <#> .
@prefix owl: <http://www.w3.org/2002/07/owl#> .
@prefix rdf: <http://www.w3.org/1999/02/22-rdf-syntax-ns#> .
@prefix xml: <http://www.w3.org/XML/1998/namespace> .
@prefix xsd: <http://www.w3.org/2001/XMLSchema#> .
@prefix rdfs: <http://www.w3.org/2000/01/rdf-schema#> .
@prefix cc: <http://creativecommons.org/ns#> .
@prefix vann: <http://purl.org/vocab/vann/> .
@prefix voaf: <http://purl.org/vocommons/voaf#> .
@prefix foaf: <http://xmlns.com/foaf/0.1/>.
@prefix schema: <http://schema.org/>.
@prefix dct: <http://purl.org/dc/terms/>.
@prefix skos: <http://www.w3.org/2004/02/skos/core#>.


#################################################################
#    Ontology Description
#################################################################

<#> a owl:Ontology ;
    dct:title "Hypermedia MAS Core Ontology"@en, "Ontologie Centrale des SMA Hypermédias"@fr ;
    dct:description  "An ontology to describe Hypermedia Multi-Agent Systems."@en,
                 "L'ontologie centrale pour la description de systèmes multi-agents hypermédias."@fr ;
    dct:issued "2021-11-21"^^xsd:date ;
    dct:contributor <http://ns.inria.fr/fabien.gandon#me> ; 
    dct:contributor <http://maxime-lefrancois.info/me#> ; 
    dct:contributor <https://danaivach.inrupt.net/profile/card#me> ; 
    dct:contributor <https://www.linkedin.com/in/christopher-leturc/> ; 
    dct:contributor <https://www.emse.fr/~boissier/> ; 
    dct:creator <http://iri.for/andrei> ;
    dct:license <http://creativecommons.org/licenses/by/3.0/> ;
    vann:preferredNamespacePrefix "hmas" ;
    vann:preferredNamespaceUri <#> .

<http://ns.inria.fr/fabien.gandon#me> a schema:Person ;
  schema:name "Fabien Gandon" ;
  schema:email "fabien.gandon@inria.fr" ;
  schema:url <http://fabien.info/> ;
  schema:identifier <http://orcid.org/0000-0003-0543-1232> ;
  schema:affiliation <https://inria.fr/> .

<https://inria.fr/> schema:name "Inria" ; schema:url <https://inria.fr/> .

<https://www.linkedin.com/in/christopher-leturc/> a schema:Person ;
  schema:name "Chistopher Leturc" ;
  schema:email "christopher.leturc@inria.fr" ;
  schema:url <https://www.linkedin.com/in/christopher-leturc/> ;
  schema:identifier <https://orcid.org/0000-0003-0821-6095> ;
  schema:affiliation <https://inria.fr/> .


<http://maxime-lefrancois.info/me#> a schema:Person ;
  schema:name "Maxime Lefrançois" ;
  schema:email "maxime.lefrancois@emse.fr" ;
  schema:url <http://maxime-lefrancois.info/> ;
  schema:identifier <http://orcid.org/0000-0001-9814-8991> ;
  schema:affiliation <https://www.mines-stetienne.fr/> .

<https://www.mines-stetienne.fr/>
  schema:name "MINES Saint-Étienne" ;
  schema:url <https://mines-stetienne.fr> .

<http://iri.for/andrei> a schema:Person ;
  schema:name "Andrei Ciortea" ;
  schema:email "andrei.ciortea@unisg.ch" ;
  schema:affiliation <https://www.unisg.ch/en>  .

<https://www.unisg.ch/en> 
  schema:name "University of St.Gallen" ; 
  schema:url <https://www.unisg.ch> .

<https://danaivach.inrupt.net/profile/card#me> a schema:Person ;
  schema:name "Danai Vachtsevanou" ;
  schema:email "danai.vachtsevanou@unisg.ch" ;
  schema:url <https://danaivach.inrupt.net/profile/card> ;
  schema:affiliation <https://www.unisg.ch/en> .

<https://www.emse.fr/~boissier/> a schema:Person ;
  schema:name "Olivier Boissier" ;
  schema:email "olivier.boissier@emse.fr" ;
  schema:affiliation <https://mines-stetienne.fr> .

#################################################################
#    Classes
#################################################################


:Agent a owl:Class ;
        rdfs:comment "An entity that is capable of autonomous behavior."@en ;
        rdfs:label "Agent"@en, "Agent"@fr ;
        rdfs:subClassOf :Hostable .

:Artifact a owl:Class ;
        rdfs:comment "A resource (or tool) that exposes affordances to agents. Agents use artifacts to achieve their design objectives."@en ;
        rdfs:label "Artifact"@en, "Artefact"@fr ;
        rdfs:subClassOf :Hostable .


:Hostable a owl:Class ;
        rdfs:comment "A resource that can be hosted on a MAS platform"@en ;
        skos:example "an agent, an artefact, other MAS platforms, workspaces, resource profiles, signifiers, organizations, can be hosted on a MAS platform"@en ;
        rdfs:label "Hostable"@en, "Hébergeable"@fr ;
        rdfs:seeAlso <https://github.com/HyperAgents/ns.hyperagents.org/issues/8> ;
        rdfs:seeAlso <https://github.com/HyperAgents/ns.hyperagents.org/issues/23> ;
        owl:disjointWith :NotHostable .




:HypermediaMASPlatform a owl:Class ;
        rdfs:comment "A Hypermedia MAS platform is a system providing a collection of features to support Hypermedia MAS. Common features include support for communication and interaction, runtime environments for agents, artifacts, or organizations, etc."@en ;
        rdfs:label "MAS Platform"@en, "Platforme SMA"@fr ;
        skos:example "Examples of hmas:HypermediaMASPlatform include Twitter, Facebook, a JADE node/delpoyment, or a JaCaMo node/delpoyment — all of which provide features that could support Hypermedia MAS & hybrid communities."@en ;
        rdfs:seeAlso <https://github.com/HyperAgents/ns.hyperagents.org/issues/20> ;
        rdfs:seeAlso <https://github.com/HyperAgents/ns.hyperagents.org/issues/32> ;
        rdfs:subClassOf :Artifact ;
        owl:disjointWith :Workspace .





:ResourceProfile a owl:Class ;
        rdfs:comment "Structured data describing a resource through general metadata, domain- and application-specific metadata, and signifiers."@en ;
        skos:example "e.g., a Thing Description document, a Hydra document, an Socio-Technical Network platform description, a fipa:AgentDescription"@en ;
        rdfs:label "Resource Profile"@en, "Profil de Ressource"@fr ;
        rdfs:subClassOf :Hostable .




:Signifier rdf:type owl:Class ;
        rdfs:comment "Structured data describing (one or multiple) affordances exposed by an artifact to agents. Structured data may include metadata about the signifier (e.g., creator, salience) or the described affordance (e.g., predicted pertinence)."@en ;
        rdfs:label "Signifier"@en, "Signifiant"@fr  ;
        skos:note ":Signifier would fit as a superclass of td:InteractionAffordance and fipa:ServiceDescription"@en ;
        skos:note ":Signifier works as a bridge between the Core and the Interaction Vocabularies."@en ;
        rdfs:seeAlso <https://github.com/HyperAgents/ns.hyperagents.org/issues/13#issuecomment-1028904491> ;
        rdfs:subClassOf :NotHostable .




:Workspace a owl:Class ;
        rdfs:comment "A logical container of one or multiple interactions among agents and potentially artifacts. Workspaces can contain any resource in general and in particular agents, artifacts, other workspaces, or platforms. A workspace can be a LDP container and this can be done by multi-typing the container or by multiple inheritance on a Class ex:Workcontainer. "@en ;
        rdfs:label "Workspace"@en, "Espace de Travail"@fr ;
        rdfs:seeAlso <https://github.com/HyperAgents/ns.hyperagents.org/issues/24> ;
        rdfs:seeAlso <https://github.com/HyperAgents/ns.hyperagents.org/issues/32> ;
        rdfs:seeAlso <https://github.com/HyperAgents/ns.hyperagents.org/issues/36> ;
        rdfs:seeAlso <https://www.w3.org/ns/ldp#> ;
        rdfs:subClassOf :Artifact ;
        owl:disjointWith :HypermediaMASPlatform .



### Top ontology constraints for coherent modeling 

# disjoint top classes 

[ a owl:AllDisjointClasses ;
    owl:members ( :Agent :Artifact :ResourceProfile :Signifier ) ] . 



#################################################################
#    Object Properties
#################################################################


:transitivelyContains a owl:TransitiveProperty ;
          owl:inverseOf :isContainedIn ;
          rdfs:domain :Workspace ;
          rdfs:range rdfs:Resource ;
          rdfs:comment "A relation that refers to all logical containers in which a resource is contained. (Never instantiate this class)"@en ;
          dct:source <https://github.com/HyperAgents/ns.hyperagents.org/issues/8#issuecomment-1025991719> ;
          rdfs:label "transitivelyContains"@en ;
          rdfs:seeAlso <https://github.com/HyperAgents/ns.hyperagents.org/issues/18> ;
          rdfs:seeAlso <https://github.com/HyperAgents/ns.hyperagents.org/issues/39> .

:directlyContains a owl:AsymmetricProperty ;
          rdfs:subPropertyOf :transitivelyContains ;
          rdfs:comment "A relation that refers to a logical containment relation and is related to the definition of a workspace as a logical container."@en ;
          dct:source <https://github.com/HyperAgents/ns.hyperagents.org/issues/18#issuecomment-1040448029> ;
          rdfs:label "directlyContains"@en .

:describes a owl:ObjectProperty ;
           owl:inverseOf :isDescribedBy ;
           rdfs:domain [ a owl:Class ;
                         owl:unionOf ( :ResourceProfile
                                       :Signifier
                                     )
                       ] ;
           rdfs:comment "A relation that describes all signifiers associated to a resource profile."@en ;
           skos:example ""@en ;
           rdfs:seeAlso <https://github.com/HyperAgents/ns.hyperagents.org/issues/13> ; 
           rdfs:seeAlso <https://github.com/HyperAgents/ns.hyperagents.org/issues/26> ;
           rdfs:label "describes"@en .



#:hasHomeMASPlatform a owl:ObjectProperty ;
#           rdfs:subPropertyOf :isHostedBy ;
#           rdfs:domain :Agent ;
#           rdfs:range :MASPlatform ;
#           rdfs:comment "The home platform of an agent is the platform on which the agent was created."@en ;
#           rdfs:seeAlso <https://github.com/HyperAgents/ns.hyperagents.org/issues/19> ;
#           rdfs:label "has home platform"@en .




#:hasHomeWorkspace a owl:ObjectProperty ;
#            rdfs:subPropertyOf :isContainedBy ;
#            owl:inverseOf :isHomeOf ;
#            rdfs:comment "The home workspace of an agent is the specific workspace where the agent spawned."@en ;
#            rdfs:seeAlso <https://github.com/HyperAgents/ns.hyperagents.org/issues/19> ;
#            rdfs:label "has home workspace"@en .


:exposesSignifier a owl:ObjectProperty ;
            rdfs:domain :ResourceProfile ;
            rdfs:range :Signifier ;
            rdfs:comment "A relation between a resource profile and a signifier"@en ;
            rdfs:label "exposes signifier"@en ;
            dct:source <https://github.com/HyperAgents/ns.hyperagents.org/issues/13#issuecomment-1029349488> ;
            rdfs:seeAlso <https://github.com/HyperAgents/ns.hyperagents.org/issues/13> .



:hosts a owl:AsymmetricProperty ;
            rdfs:domain :HypermediaMASPlatform ;
            rdfs:range :Hostable ;
            rdfs:comment "A relation that refers to an information resource or a process (e.g., agent) that is hosted on a platform. A hosting relation might have further implications, e.g. the usage of the hosted resource (or the usage of platform resources by the hosted resource) could be subject to terms of service or data licensing policies specific to the hosting platform."@en ;
            rdfs:label "hosts"@en ;
            dct:source <https://github.com/HyperAgents/ns.hyperagents.org/issues/8#issuecomment-1025991719> ;
            rdfs:seeAlso <https://github.com/HyperAgents/ns.hyperagents.org/issues/18> .



:isContainedIn a owl:AsymmetricProperty ;
            rdfs:range :Workspace ;
            rdfs:comment "A relation that describes the workspace that contains a resource."@en ;
            rdfs:label "is contained in"@en .


:isDescribedBy a owl:AsymmetricProperty ;
            rdfs:range [ a owl:Class ;
                            owl:unionOf ( :ResourceProfile
                                          :Signifier
                                        )
                          ] ;
            rdfs:comment "A relation which maps the resource profiles and signifiers associated to a resource."@en ;
            rdfs:label "is described by"@en .


:isHomeOf a owl:AsymmetricProperty ;
            rdfs:domain :Workspace ;
            rdfs:range :Agent ;
            rdfs:comment "The home workspace is the specific workspace where the agent spawned"@en ;
            rdfs:label "is home of"@en .




:isHostedBy a owl:AsymmetricProperty ; 
            owl:inverseOf :hosts ;
            rdfs:domain :Hostable ;
            rdfs:range :HypermediaMASPlatform ;
            rdfs:comment "A relations that refers to the platform that hosts the resource. "@en ;
            rdfs:label "is hosted by"@en .

