@base <https://purl.org/hmas/> .
@prefix : <> .
@prefix owl: <http://www.w3.org/2002/07/owl#> .
@prefix rdf: <http://www.w3.org/1999/02/22-rdf-syntax-ns#> .
@prefix xml: <http://www.w3.org/XML/1998/namespace> .
@prefix xsd: <http://www.w3.org/2001/XMLSchema#> .
@prefix rdfs: <http://www.w3.org/2000/01/rdf-schema#> .
@prefix vann: <http://purl.org/vocab/vann/> .

:fipa rdf:type owl:Ontology ;
    owl:imports :core ;
    vann:preferredNamespacePrefix "hmas" ;
    vann:preferredNamespaceUri <> .

#################################################################
#    Object Properties
#################################################################

###  https://ci.mines-stetienne.fr/fipa#hasServiceName
:hasServiceName rdf:type owl:ObjectProperty ;
                rdfs:isDefinedBy :fipa ;
                rdfs:domain :APService ;
                rdfs:label "has Service Name"@en .


###  https://ci.mines-stetienne.fr/fipa#hasServiceType
:hasServiceType rdf:type owl:ObjectProperty ;
                rdfs:isDefinedBy :fipa ;
                rdfs:domain :APService ;
                rdfs:label "has Service Type"@en .


#################################################################
#    Classes
#################################################################

###  https://ci.mines-stetienne.fr/fipa#APService
:APService rdf:type owl:Class ;
           rdfs:isDefinedBy :fipa ;
           rdfs:comment "A service exposed by a FIPA Agent Platform as defined by the FIPA Abstract Architecture Specification (http://fipa.org/specs/fipa00001/SC00001L.html)."@en ;
           rdfs:label "Agent Platform Service"@en .


###  https://ci.mines-stetienne.fr/fipa#AgentIdentifierDescription
:AgentIdentifierDescription rdf:type owl:Class ;
                            rdfs:isDefinedBy :fipa ;
                            rdfs:subClassOf <https://ci.mines-stetienne.fr/hmas#ResourceProfile> ;
                            rdfs:comment "A resource profile that describes an agent using the Agent Identifier Description defined by the FIPA Agent Management Specification (http://fipa.org/specs/fipa00023/SC00023K.html)."@en ;
                            rdfs:label "Agent Identifier Description"@en .


###  https://ci.mines-stetienne.fr/fipa#AgentPlatformDescription
:AgentPlatformDescription rdf:type owl:Class ;
                          rdfs:isDefinedBy :fipa ;
                          rdfs:subClassOf <https://ci.mines-stetienne.fr/hmas#ResourceProfile> ;
                          rdfs:comment "A resource profile that descripe a FIPA Agent Platform using the Agent Platform Description defined by the FIPA Agent Management Specification (http://fipa.org/specs/fipa00023/SC00023K.html)."@en ;
                          rdfs:label "Agent Platform Description"@en .


###  https://ci.mines-stetienne.fr/fipa#FIPAAgentPlatform
:FIPAAgentPlatform rdf:type owl:Class ;
                   rdfs:isDefinedBy :fipa ;
                   rdfs:subClassOf <https://ci.mines-stetienne.fr/hmas#Platform> ;
                   rdfs:comment "A platform that conforms to the FIPA Abstract Architecture Specification (http://fipa.org/specs/fipa00001/SC00001L.html)."@en ;
                   rdfs:label "FIPA Agent Platform"@en .


###  https://ci.mines-stetienne.fr/fipa#HTTPMessageTransportService
:HTTPMessageTransportService rdf:type owl:Class ;
                             rdfs:isDefinedBy :fipa ;
                             rdfs:subClassOf :MessageTransportService ;
                             rdfs:comment "An HTTP-based message transport service that confirms to the FIPA Agent Message Transport Protocol for HTTP Specification (http://fipa.org/specs/fipa00084/SC00084F.html)."@en ;
                             rdfs:label "HTTP Message Transport Service"@en .


###  https://ci.mines-stetienne.fr/fipa#IIOPMessageTransportService
:IIOPMessageTransportService rdf:type owl:Class ;
                             rdfs:isDefinedBy :fipa ;
                             rdfs:subClassOf :MessageTransportService ;
                             rdfs:comment "An HTTP-based message transport service that confirms to the FIPA Agent Message Transport Protocol for IIOP Specification (http://fipa.org/specs/fipa00075/SC00075G.html)."@en ;
                             rdfs:label "IIOP Message Transport Service"@en .


###  https://ci.mines-stetienne.fr/fipa#MessageTransportService
:MessageTransportService rdf:type owl:Class ;
                         rdfs:isDefinedBy :fipa ;
                         rdfs:subClassOf :APService ;
                         rdfs:comment "A service for transporting messages among agents that conforms to the FIPA Message Transport Service Specification (http://fipa.org/specs/fipa00067/SC00067F.html)."@en ;
                         rdfs:label "Message Transport Service"@en .


###  Generated by the OWL API (version 4.5.9.2019-02-01T07:24:44Z) https://github.com/owlcs/owlapi

:failure rdf:type :CommunicativeAct ;
         rdfs:isDefinedBy :fipa ;
         rdfs:comment "A communicative act with which the sender fails to perform some action"@en ;
         rdfs:label "failure"@en .

:informDone rdf:type :CommunicativeAct ;
         rdfs:isDefinedBy :fipa ;
         rdfs:comment "A communicative act with which the sender informs a requested action has been done"@en ;
         rdfs:label "inform done"@en .

:informResult rdf:type :CommunicativeAct ;
         rdfs:isDefinedBy :fipa ;
         rdfs:comment "A communicative act with which the sender informs the progress concerning a requested action"@en ;
         rdfs:label "inform result"@en .
