@base <https://ci.mines-stetienne.fr/fna> .
@prefix : <#> .
@prefix owl: <http://www.w3.org/2002/07/owl#> .
@prefix rdf: <http://www.w3.org/1999/02/22-rdf-syntax-ns#> .
@prefix xml: <http://www.w3.org/XML/1998/namespace> .
@prefix xsd: <http://www.w3.org/2001/XMLSchema#> .
@prefix rdfs: <http://www.w3.org/2000/01/rdf-schema#> .
@prefix time: <http://www.w3.org/2006/time#> .

<#> rdf:type owl:Ontology ;
                                       owl:imports <https://ci.mines-stetienne.fr/hmas#> .





#################################################################
#    Classes
#################################################################

###  https://ci.mines-stetienne.fr/fna#NormativeRule
:Norm rdf:type owl:Class ;
           rdfs:comment "A norm specification associated to a resource"@en ;
           rdfs:label "Norm"@en .

:NormPrecondition rdf:type owl:Class ;
           rdfs:comment "A precondition specification associated to a norm to be applied"@en ;
           rdfs:label "Norm"@en .
           
:NormSpecification rdf:type owl:Class ;
           rdfs:comment "A specification described the content of a norm when a context (preconditions) is verified"@en ;
           rdfs:label "Norm"@en .

:PossibleFact rdf:type owl:Class ;
           rdfs:comment "A possible fact describes a possible information about the real world that may occure or not"@en ;
           rdfs:label "Possible fact"@en .

:ProvedFact rdf:type owl:Class ;
	   rdfs:subClassOf :PossibleFact ;
           rdfs:comment "A proved fact describes a possible information that has been proved"@en ;
           rdfs:label "Proved fact"@en .        
           
#:ContextualFact rdf:type owl:Class ; 
#	    rdfs:subClassOf :PossibleFact ;
#           rdfs:comment "A context describes a fac"@en ;
#           rdfs:label "Fact"@en .



:Modality rdf:type owl:Class ;
           rdfs:comment "A modality may be associated to a ressource (e.g. belief, desire, intention, obligation, permission, etc.)"@en ;
           rdfs:label "Modal type"@en .

:Effect rdf:type owl:Class ; 
	   rdfs:subClassOf :Modality ;
           rdfs:comment "An effect modality refers to a consequence of an action "@en ;
           rdfs:label "Effect"@en .

:DeliberateEffect rdf:type owl:Class ; 
	   rdfs:subClassOf :Modality ;
           rdfs:comment "An effect that has been deliberated by an agent"@en ;
           rdfs:label "Deliberate Effect"@en .

:DoxasticModality rdf:type owl:Class ; 
	   rdfs:subClassOf :Modality ;
           rdfs:comment "A doxastic modality refers to an abstract type associated to belief "@en ;
           rdfs:label "Belief"@en .

:DeonticModality rdf:type owl:Class ; 
	   rdfs:subClassOf :Modality ;
           rdfs:comment "A deontic modality refers to an abstract type associated to obligation, neutral, prohibition or permission "@en ;
           rdfs:label "Deontic duty"@en .

:Obligation rdf:type owl:Class ; 
	   rdfs:subClassOf :Modality ;
           rdfs:comment "Obligation is deontic modal type associated with obligation (duty)"@en ;
           rdfs:label "Obligation"@en .


:Permission rdf:type owl:Class ; 
	   rdfs:subClassOf :Modality ;
           rdfs:comment "Right is deontic modal type associated with permission (right)"@en ;
           rdfs:label "Permission"@en .

:Prohibition rdf:type owl:Class ; 
	   rdfs:subClassOf :Modality ;
           rdfs:comment " is deontic modal type associated with prohibition (no-right)"@en ;
           rdfs:label "Prohibition"@en .

:Neutrality rdf:type owl:Class ; 
	   rdfs:subClassOf :Modality ;
           rdfs:comment "Neutrality is deontic modal type associated with a not obligatory, and not prohibited fact (i.e. contingent or privilege)"@en ;
           rdfs:label "Neutrality"@en .
           
           
:InterpretationMode rdf:type owl:Class ; 
           rdfs:comment "Interpretation mode describes a formal mode to interprete a resource. (e.g. "@en ;
           rdfs:label "Neutrality"@en .

:ExegenetiqueInterpretation rdf:type owl:Class ; 
	   rdfs:subClassOf :InterpretationMode ;
           rdfs:comment "A law is interpreted through a linguistical approach"@en ;
           rdfs:label "Social interpretation"@en .         
      
:AnalogousInterpretation rdf:type owl:Class ; 
   rdfs:subClassOf :InterpretationMode ;
   rdfs:comment "A law is interpreted through past application cases which are closed"@en ;
   rdfs:label "Social interpretation"@en .   
           
:SocialInterpretation rdf:type owl:Class ; 
	   rdfs:subClassOf :InterpretationMode ;
           rdfs:comment "A law is interpreted through a social context"@en ;
           rdfs:label "Social interpretation"@en .
           
:LegalApplication rdf:type owl:Class ; 
           rdfs:comment "A legal application corresponds to typical effects of the application of legal norms  (e.g. power, liability, disability, immunity)"@en ;
           rdfs:label "Legal Application"@en .
        
        
   
:ViolationCase rdf:type owl:Class ; 
           rdfs:comment "Violation case states what is a typical case of violation for a given norm"@en ;
           rdfs:label "Violation Case"@en .

:PunishmentCase rdf:type owl:Class ; 
           rdfs:comment "Punishment case states a sanction associated with a violation of a norm"@en ;
           rdfs:label "Punishment case"@en .


#################################################################
#    Object Properties
#################################################################




###  https://ci.mines-stetienne.fr/fna#hasNorm
:doesNotRespectNorm rdf:type owl:ObjectProperty ;
                rdfs:range :Norm ;
                rdfs:comment "Associates a norm which is violated by a resource"@en ;
                rdfs:label "does not respect the norm"@en .


###  https://ci.mines-stetienne.fr/fna#hasAViolationCase
:hasAViolationCase rdf:type owl:ObjectProperty ;
		rdfs:domain :Norm ;
                rdfs:range :ViolationCase ;
                rdfs:comment "Associates cases of violation of a norm"@en ;
                rdfs:label "has a violation case"@en .

###  https://ci.mines-stetienne.fr/fna#hasNorm
:hasPunishmentCase rdf:type owl:ObjectProperty ;
                rdfs:domain :Norm ;
               	rdfs:range :PunishmentCase ;
                rdfs:comment "Associates a norm to a punishment in case of violation"@en ;
                rdfs:label "has punishment"@en .

###  https://ci.mines-stetienne.fr/fna#statedAs
:statedAs rdf:type owl:ObjectProperty ;
                rdfs:range :Modality ;
                rdfs:comment "The resource is stated with a certain modality"@en ;
                rdfs:label "is stated as"@en .

   
###  https://ci.mines-stetienne.fr/fna#occurred            
:occurred rdf:type owl:ObjectProperty ;
		rdfs:domain :PossibleFact ;
                rdfs:range time:TemporalEntity ;
                rdfs:comment "A relation that describes when a possible fact possibly occurred"@en ;
                rdfs:label "has norm"@en .

###  https://ci.mines-stetienne.fr/fna#occurred            
:relatedEvidence rdf:type owl:ObjectProperty ;
		rdfs:domain :ProvedFact ;
                rdfs:range :ProvedFact ;
                rdfs:comment "A relation that describes which are the related evidences associated to a proved fact"@en ;
                rdfs:label "has norm"@en .

                 
                
###  https://ci.mines-stetienne.fr/fna#hasNormPrecondition
:hasNormPrecondition rdf:type owl:ObjectProperty ;
		rdfs:domain :Norm ;
                rdfs:range :ContextualFact ;
                rdfs:comment "A resource may be associated to a normative rule"@en ;
                rdfs:label "has Normative Rule"@en .  


###  https://ci.mines-stetienne.fr/fna#hasNormSpecification
:hasNormSpecification rdf:type owl:ObjectProperty ;
		rdfs:domain :Norm ;
                rdfs:range :NormSpecification ;
                rdfs:comment "A resource may be associated to a normative rule"@en ;
                rdfs:label "has Normative Rule"@en . 
                
                
                 
                

