@base <https://purl.org/hmas/> .
@prefix : <> .
@prefix owl: <http://www.w3.org/2002/07/owl#> .
@prefix xsd: <http://www.w3.org/2001/XMLSchema#> .
@prefix rdfs: <http://www.w3.org/2000/01/rdf-schema#> .
@prefix cc: <http://creativecommons.org/ns#> .
@prefix vann: <http://purl.org/vocab/vann/> .
@prefix dct: <http://purl.org/dc/terms/>.
@prefix sh: <http://www.w3.org/ns/shacl#> .

#################################################################
#    Ontology Description
#################################################################

:interaction a owl:Ontology ;
    owl:imports :core ;
    dct:title "Hypermedia MAS Interaction Ontology"@en, "Ontologie d'Interaction des SMA Hypermédias"@fr ;
    dct:description "An ontology to describe interaction in Hypermedia Multi-Agent Systems."@en, 
                  "L'ontologie pour décrire l'interaction dans les systèmes multi-agents hypermédias."@fr ;
    dct:issued "2023-01-13"^^xsd:date ;
    cc:license <https://creativecommons.org/licenses/by/4.0/> ;
    dct:creator <https://danaivach.inrupt.net/profile/card#me> ;
    dct:contributor <https://pod.inrupt.com/andreiciortea/profile/card#me> ;
    dct:contributor <https://pod.inrupt.com/smnmyr/profile/card#me> ;
    dct:contributor <http://ns.inria.fr/fabien.gandon#me> ; 
    cc:license <https://creativecommons.org/licenses/by/4.0/> ;
    vann:preferredNamespacePrefix "hmas" ;
    vann:preferredNamespaceUri <> .

#################################################################
#    Classes
#################################################################

:ActionExecution a owl:Class ;
                 rdfs:isDefinedBy :interaction ;
                 rdfs:subClassOf :BehaviorExecution ;
                 rdfs:comment "A behavior execution that is the execution of exactly one context-free action, e.g. of a context-free HTTP request."@en ;
                 rdfs:label "action execution"@en,  "exécution de l'action"@fr .

:BehaviorExecution a owl:Class ;
                   rdfs:isDefinedBy :interaction ;
                   rdfs:comment "A course of action performed by an agent upon exploiting a behavior possibility."@en ;
                   rdfs:label "behavior execution"@en, "exécution du comportement"@fr .

:Input a owl:Class ;
       rdfs:isDefinedBy :interaction ;
       rdfs:comment "An input of an action, for example, in the representation of an action execution."@en ;
       rdfs:label "input"@en, "entrée"@fr .

#################################################################
#    Object Properties
#################################################################

:hasInput a owl:ObjectProperty ;
              rdfs:isDefinedBy :interaction ;
              rdfs:domain :ActionExecution ;
              rdfs:range :Input ;
              rdfs:comment "A relation between an action execution and the input that it has."@en ;
              rdfs:label "has input"@en, "a une entrée"@fr .

:signifies a owl:ObjectProperty ;
           rdfs:isDefinedBy :interaction ;
           rdfs:domain :Signifier ;
           rdfs:range sh:NodeShape ;
           rdfs:comment "A relation between a signifier and a node shape specifying a description of the expected behavior execution."@en ;
           rdfs:label "signifies"@en, "signifie"@fr .
