@base <https://purl.org/hmas/> .
@prefix : <> .
@prefix owl: <http://www.w3.org/2002/07/owl#> .
@prefix rdf: <http://www.w3.org/1999/02/22-rdf-syntax-ns#> .
@prefix xml: <http://www.w3.org/XML/1998/namespace> .
@prefix xsd: <http://www.w3.org/2001/XMLSchema#> .
@prefix rdfs: <http://www.w3.org/2000/01/rdf-schema#> .
@prefix cc: <http://creativecommons.org/ns#> .
@prefix vann: <http://purl.org/vocab/vann/> .
@prefix voaf: <http://purl.org/vocommons/voaf#> .
@prefix foaf: <http://xmlns.com/foaf/0.1/>.
@prefix schema: <http://schema.org/>.
@prefix dct: <http://purl.org/dc/terms/>.
@prefix skos: <http://www.w3.org/2004/02/skos/core#>.

#################################################################
#    Ontology Description
#################################################################

:interaction a owl:Ontology ;
    owl:imports :core ;
    dct:title "Hypermedia MAS Interaction Ontology"@en, "Ontologie d'Interaction des SMA Hypermédias"@fr ;
    dct:description "An ontology to describe interaction in Hypermedia Multi-Agent Systems."@en, 
                  "L'ontologie pour décrire l'interaction dans les systèmes multi-agents hypermédias."@fr ;
    dct:issued "2023-01-13"^^xsd:date ;
    cc:license <https://creativecommons.org/licenses/by/4.0/> ;
    dct:creator <https://danaivach.inrupt.net/profile/card#me> ;
    dct:contributor <https://pod.inrupt.com/andreiciortea/profile/card#me> ;
    dct:contributor <https://pod.inrupt.com/smnmyr/profile/card#me> ;
    cc:license <https://creativecommons.org/licenses/by/4.0/> ;
    vann:preferredNamespacePrefix "hmas" ;
    vann:preferredNamespaceUri <> .

#################################################################
#    Classes
#################################################################

:ActionExecution a owl:Class ;
                 rdfs:isDefinedBy :interaction ;
                 rdfs:subClassOf :BehaviorExecution ;
                 rdfs:comment "A behavior execution that is the execution of exactly one context-free action, e.g. of a context-free HTTP request."@en ;
                 rdfs:label "action execution"@en .

:ActionSpecification a owl:Class ;
                     rdfs:isDefinedBy :interaction ;
                     rdfs:subClassOf :BehaviorSpecification ;
                     rdfs:comment "A specification that describes an action (e.g., through preconditions and postconditions) and how to execute the action, e.g. as a context-free request through a form."@en ;
                     rdfs:label "action specification"@en .

:BehaviorExecution a owl:Class ;
                   rdfs:isDefinedBy :interaction ;
                   rdfs:comment "A course of action performed by an agent upon exploiting a behavior possibility."@en ;
                   rdfs:label "behavior execution"@en .

:BehaviorSpecification a owl:Class ;
                       rdfs:isDefinedBy :interaction ;
                       rdfs:comment "A specification that describes a behavior, for example, as procedural knowledge (e.g., AgentSpeak plan) or code-on-demand (e.g., a script that implements a behavior)."@en ;
                       rdfs:label "behavior specification"@en .

:Input a owl:Class ;
       rdfs:isDefinedBy :interaction ;
       rdfs:comment "An input of an action, which may include variables. The input may be used, for instance, in an action specification or in the representation of an action execution."@en ;
       rdfs:label "input"@en .

#################################################################
#    Object Properties
#################################################################

:expectsInput a owl:ObjectProperty ;
              rdfs:isDefinedBy :interaction ;
              rdfs:domain :ActionSpecification ;
              rdfs:range :Input ;
              rdfs:comment "A relation between an action specification and the input that the specified action expects."@en ;
              rdfs:label "expects input"@en .

:hasForm a owl:ObjectProperty ;
         rdfs:isDefinedBy :interaction ;
         rdfs:domain :ActionSpecification ;
         rdfs:comment "A relation between an action specification and a form that describes how to execute the specified action."@en ;
         rdfs:label "has form"@en .

:hasSchema a owl:ObjectProperty ;
           rdfs:isDefinedBy :interaction ;
           rdfs:comment "A relation between an input and the schema of the input."@en ;
           rdfs:label "has schema"@en .

:signifies a owl:ObjectProperty ;
           rdfs:isDefinedBy :interaction ;
           rdfs:domain :Signifier ;
           rdfs:range :BehaviorSpecification ;
           rdfs:comment "A relation between a signifier and a behavior specification it signifies."@en ;
           rdfs:label "signifies"@en .
