@base <https://purl.org/hmas/> .
@prefix : <> .
@prefix owl: <http://www.w3.org/2002/07/owl#> .
@prefix rdf: <http://www.w3.org/1999/02/22-rdf-syntax-ns#> .
@prefix xml: <http://www.w3.org/XML/1998/namespace> .
@prefix xsd: <http://www.w3.org/2001/XMLSchema#> .
@prefix rdfs: <http://www.w3.org/2000/01/rdf-schema#> .
@prefix sh: <http://www.w3.org/ns/shacl#> .
@prefix vann: <http://purl.org/vocab/vann/> .

:jason-kqml rdf:type owl:Ontology ;
    owl:imports :core, :interaction ;
    vann:preferredNamespacePrefix "hmas" ;
    vann:preferredNamespaceUri <> .

#################################################################
#    Object Properties
#################################################################

:hasPerformative rdf:type owl:ObjectProperty ;
                 rdfs:isDefinedBy :jason-kqml ;
                 rdfs:range :CommunicativeAct ;
                 rdfs:comment "A relation between a message and the communicative act of the message."@en ;
                 rdfs:label "has performative"@en .


:hasReceiver rdf:type owl:ObjectProperty ;
             rdfs:isDefinedBy :jason-kqml ;
             rdfs:range :Agent ;
             rdfs:comment "A relation between a message and agents that are the intended recipients of the message."@en ;
             rdfs:label "has receiver"@en .


:hasSender rdf:type owl:ObjectProperty ;
           rdfs:isDefinedBy :jason-kqml ;
           rdfs:range :Agent ;
           rdfs:comment "A relation between a message and the agent that is the sender of the message."@en ;
           rdfs:label "has sender"@en .


:hasContent rdf:type owl:ObjectProperty ;
           rdfs:isDefinedBy :jason-kqml ;
           rdfs:comment "A relation between a message and the content of the message."@en ;
           rdfs:label "has content"@en .


:hasLanguage rdf:type owl:ObjectProperty ;
             rdfs:isDefinedBy :jason-kqml ;
             rdfs:range :Language ;
             rdfs:comment "A relation between a message and the language in which the message content parameter is expressed."@en ;
             rdfs:label "has language"@en .


#################################################################
#    Classes
#################################################################

:CommunicativeAct rdf:type owl:Class ;
                  rdfs:isDefinedBy :jason-kqml ;
                  rdfs:comment "A KQML communicative act that can be used as a performative for communicating with Jason agents."@en ;
                  rdfs:label "KQML Communicative Act"@en .


:ACLMessage rdf:type owl:Class ;
            rdfs:isDefinedBy :jason-kqml ;
            rdfs:comment "A message that uses the KQML Agent Communication Language and that can be used for communication Jason agents."@en ;
            rdfs:label "ACL Message"@en .


:Language rdf:type owl:Class ;
          rdfs:isDefinedBy :jason-kqml ;
          rdfs:comment "The language in which the content of a message is expressed, for example, the AgentSpeak language"@en ;
          rdfs:label "Language"@en .


#################################################################
#    Individuals
#################################################################

:AgentSpeak rdf:type :Language ;
        rdfs:isDefinedBy :jason-kqml ;
        rdfs:comment "The AgentSpeak language"@en ;
        rdfs:label "AgentSpeak"@en .

:tell rdf:type :CommunicativeAct ;
      rdfs:isDefinedBy :jason-kqml ;
      rdfs:comment "A communicative act with which the sender intends the receiver to believe (that the sender believes) the literal in the message’s content to be true."@en ;
      rdfs:label "tell"@en .

:untell rdf:type :CommunicativeAct ;
        rdfs:isDefinedBy :jason-kqml ;
        rdfs:comment "A communicative act with which the sender intends the receiver not to believe (that the sender believes) the literal in the message’s content to be true."@en ;
        rdfs:label "untell"@en .

:achieve rdf:type :CommunicativeAct ;
         rdfs:isDefinedBy :jason-kqml ;
         rdfs:comment "A communicative act with which the sender requests the receiver to try and achieve a state of affairs where the literal in the message content is true (i.e. the sender is delegating a goal to the receiver)."@en ;
         rdfs:label "acheive"@en .

:unachieve rdf:type :CommunicativeAct ;
           rdfs:isDefinedBy :jason-kqml ;
           rdfs:comment "A communicative act with which the sender requests the receiver to drop the goal of achieving a state of affairs where the message content is true."@en ;
           rdfs:label "unachieve"@en .

:askOne rdf:type :CommunicativeAct ;
        rdfs:isDefinedBy :jason-kqml ;
        rdfs:comment "A communicative act with which the sender wants to know if the content of the message is true for the receiver (i.e. if there is an answer that makes the content a logical consequence of the receiver’s belief base, by appropriate substitution of variables)."@en ;
        rdfs:label "askOne"@en .

:askAll rdf:type :CommunicativeAct ;
        rdfs:isDefinedBy :jason-kqml ;
        rdfs:comment "A communicative act with which the sender wants all of the receiver’s answers to a question."@en ;
        rdfs:label "askAll"@en .

:tellHow rdf:type :CommunicativeAct ;
         rdfs:isDefinedBy :jason-kqml ;
         rdfs:comment "A communicative act with which the sender informs the receiver of a plan (the sender’s know-how)."@en ;
         rdfs:label "tellHow"@en .

:untellHow rdf:type :CommunicativeAct ;
           rdfs:isDefinedBy :jason-kqml ;
           rdfs:comment "A communicative act with which the sender requests the receiver to disregard a certain plan (i.e. delete that plan from its plan library)."@en ;
           rdfs:label "untellHow"@en .

:askHow rdf:type :CommunicativeAct ;
        rdfs:isDefinedBy :jason-kqml ;
        rdfs:comment "A communicative act with which the sender wants all of the receiver’s plans that are relevant for the triggering event in the message content."@en ;
        rdfs:label "askHow"@en .


