@base <https://purl.org/meta> .
@prefix : <#> .
@prefix owl: <http://www.w3.org/2002/07/owl#> .
@prefix rdf: <http://www.w3.org/1999/02/22-rdf-syntax-ns#> .
@prefix xml: <http://www.w3.org/XML/1998/namespace> .
@prefix xsd: <http://www.w3.org/2001/XMLSchema#> .
@prefix rdfs: <http://www.w3.org/2000/01/rdf-schema#> .
@prefix cc: <http://creativecommons.org/ns#> .
@prefix vann: <http://purl.org/vocab/vann/> .
@prefix voaf: <http://purl.org/vocommons/voaf#> .
@prefix foaf: <http://xmlns.com/foaf/0.1/>.
@prefix schema: <http://schema.org/> .
@prefix dct: <http://purl.org/dc/terms/> .
@prefix skos: <http://www.w3.org/2004/02/skos/core#> .
#@prefix doco: <http://purl.org/spar/doco#> .

<#> rdf:type owl:Ontology ;
                                       owl:imports <https://purl.org/meta#> .

:Issue a owl:Annotation ;
        skos:definition "An Issue is a tracking tool that is integrated with your GitHub repository to track ideas, work, and bugs without leaving GitHub."@en ;
        rdfs:seeAlso <https://github.com/features/issues> ;
        rdfs:label "Issue"@en .

:MotivatingScenario a owl:Annotation ;
        skos:definition "A Motivating Scenario (MS) is a small story problem that provides a short description and a set of informal and intuitive examples to the problem it talks about."@en ;
        rdfs:seeAlso <https://essepuntato.it/samod/> ;
        dcterms:source <http://dx.doi.org/10.1109/MIS.2002.999223> ;
        rdfs:label "MotivatingScenario"@en .

:InformalCompetencyQuestion a owl:Annotation ;
        skos:definition "An Informal Competency Question (ICQ) is a natural language question that represents an informal requirement within a particular domain."@en ;
        dcterms:source <http://dx.doi.org/10.1109/MIS.2002.999223> ;
        rdfs:label "InformalCompetencyQuestion"@en .

[ a owl:AllDisjointClasses ;
    owl:members ( :Issue :MotivatingScenario :InformalCompetencyQuestion ) ] . 

:hasIssue rdf:type owl:AnnotationProperty, owl:AsymmetricProperty ;
                rdfs:range :Issue ;
                rdfs:label "has issue"@en .

:hasMS rdf:type owl:AnnotationProperty, owl:AsymmetricProperty ;
                rdfs:range :MotivatingScenario ;
                rdfs:label "has MS"@en .

:answersTheICQ rdf:type owl:AnnotationProperty ;
                rdfs:domain :MotivatingScenario ;
                rdfs:range :InformalCompetencyQuestion ;
                rdfs:label "answers the ICQ"@en .

:hasGlossary rdf:type owl:AnnotationProperty ;
                rdfs:domain :MotivatingScenario ;
                rdfs:range doco:Glossary;
                rdfs:label "has a glossary"@en .
