@base <https://purl.org/hmas/> .
@prefix : <> .
@prefix owl: <http://www.w3.org/2002/07/owl#> .
@prefix rdf: <http://www.w3.org/1999/02/22-rdf-syntax-ns#> .
@prefix xml: <http://www.w3.org/XML/1998/namespace> .
@prefix xsd: <http://www.w3.org/2001/XMLSchema#> .
@prefix rdfs: <http://www.w3.org/2000/01/rdf-schema#> .
@prefix cc: <http://creativecommons.org/ns#> .
@prefix vann: <http://purl.org/vocab/vann/> .
@prefix voaf: <http://purl.org/vocommons/voaf#> .
@prefix foaf: <http://xmlns.com/foaf/0.1/> .
@prefix schema: <http://schema.org/> .
@prefix dct: <http://purl.org/dc/terms/> .
@prefix skos: <http://www.w3.org/2004/02/skos/core#> .

#################################################################
#    Ontology Description
#################################################################

:regulation rdf:type owl:Ontology ;
    dct:title "Hypermedia MAS Regulation Ontology"@en, "Ontologie de Régulation des SMA Hypermédias"@fr ;
    dct:description "An ontology to describe the regulation of Hypermedia Multi-Agent Systems."@en, "L'ontologie pour décrire la régulation des systèmes multi-agents hypermédias."@fr ;
    dct:issued "2022-05-01"^^xsd:date ;
    dct:modified "2024-05-27"^^xsd:date ;
    owl:imports :core ;
    dct:creator <https://orcid.org/0000-0002-4506-2745> ;
    dct:contributor <https://orcid.org/0000-0002-2956-0533> ; 
    dct:contributor <https://orcid.org/0000-0003-0821-6095>  ; 
    dct:contributor <https://danaivach.inrupt.net/profile/card#me> ;
    dct:contributor <http://ns.inria.fr/fabien.gandon#me> ;
    dct:contributor <http://maxime-lefrancois.info/me#> ;
    dct:contributor <https://orcid.org/0000-0003-4509-9537> ;
    dct:contributor <https://orcid.org/0000-0002-3497-8758> ;
    cc:license <https://creativecommons.org/licenses/by/4.0/> ;
    vann:preferredNamespacePrefix "hmas" ;
    vann:preferredNamespaceUri <> .

#################################################################
#    Concepts
#################################################################

:OrganizationModel a skos:Concept ;
    skos:prefLabel "organization model"@en ;
    skos:definition "An Organization Model is the combination of Roles, Organizational Goals, and Facilities in a consistent way used to enact one or multiple Organizations."@en ;
    skos:editorialNote "The Organization Model is represented as SHACL Shapes."@en ;
    skos:related :Organization .

#################################################################
#    Classes
#################################################################
       
:Role a owl:Class ;
    rdfs:isDefinedBy :regulation ;
    rdfs:comment "A Role defines positions of members (i.e., Agents) in an Organization."@en ;
    rdfs:label "role"@en, "rôle"@fr .

:OrganizationalGoal a owl:Class ;
    rdfs:isDefinedBy :regulation ;
    rdfs:comment "An Organizational Goal is a pursued state of affairs."@en ;
    rdfs:label "organizational goal"@en, "but organisationnel"@fr .
    
:Facility a owl:Class ;
    rdfs:isDefinedBy :regulation ;
    rdfs:comment "A Facility defines functions of materials (i.e., Artifacts) in an Organization."@en ;
    rdfs:label "facility"@en, "facilité"@fr .

:OrganizationalValue a owl:Class ;
    rdfs:isDefinedBy :regulation ;
    rdfs:comment "An Organizational Value is a belief about socially or personally desirable end state or action that are explicitly or implicitly shared by members of an Organization."@en ;
    rdfs:label "organizational value"@en, "valeur organisationnelle"@fr .

:Membership a owl:Class ;
    rdfs:isDefinedBy :regulation ;
    rdfs:comment "A Membership indicates the Role played by an Agent in a Group of an Organization." ;
    rdfs:label "membership"@en, "l'appartenance"@fr .
    
:Group a owl:Class ;
    rdfs:isDefinedBy :regulation ;
    rdfs:comment "A Group is a subset of Agents in an Organization that belong together."@en ;
    skos:example "In a human organization, a HR department is seen as a group." ;
    rdfs:label "group"@en, "groupe"@fr .

:Mission a owl:Class ;
    rdfs:isDefinedBy :regulation ;
    rdfs:comment "A set of duties that Agents can commit to for achieving Organizational Goals."@en ;
    rdfs:label "mission"@en, "mission"@fr .

:Process a owl:Class ;
    rdfs:isDefinedBy :regulation ;
    rdfs:comment "A plan specified as a set of Missions to be executed by several coordinating Agents."@en ;
    rdfs:label "process"@en, "processus"@fr .

:Commitment a owl:Class ;
    rdfs:isDefinedBy :regulation ;
    rdfs:comment "A Commitment is an engagement of an Agent with the duties of a Mission."@en ;
    rdfs:label "commitment"@en, "engagement"@fr .

:Usage a owl:Class ;
    rdfs:isDefinedBy :regulation ;
    rdfs:comment "A set of Facilities that Agents can use in a Setting."@en ;
    rdfs:label "usage"@en, "usage"@fr .
    
:Setting a owl:Class ;
    rdfs:isDefinedBy :regulation ;
    rdfs:comment "A Setting is the context in which a Usage is set."@en ;
    rdfs:label "setting"@en, "contexte d'usage"@fr .

:Access a owl:Class ;
    rdfs:isDefinedBy :regulation ;
    rdfs:comment "An opportunity an Agent have to use an Artifact in the context of a Usage."@en ;
    rdfs:label "access"@en, "accès"@fr .
    
#################################################################
#    Object Properties
#################################################################

:proposesRole a owl:ObjectProperty ;
    rdfs:isDefinedBy :regulation ;
    rdfs:domain :Organization ;
    rdfs:range :Role ;
    rdfs:isDefinedBy :regulation ;
    rdfs:comment "A relation that refers to a Role made available to Agents in the context of an Organization."@en ;
    rdfs:label "proposes role"@en, "fournit un rôle"@fr .

:hasOrganizationalGoal a owl:ObjectProperty ;
    rdfs:isDefinedBy :regulation ;
    rdfs:domain :Organization ;
    rdfs:range :OrganizationalGoal ;
    rdfs:comment "A relation that refers to an Organizational Goal of an Organization."@en ;
    rdfs:label "has organizational goal"@en, "a un but organisationnel"@fr .
    
:proposesFacility a owl:ObjectProperty ;
    rdfs:isDefinedBy :regulation ;
    rdfs:domain :Organization ;
    rdfs:range :Facility ;
    rdfs:comment "A relation that refers to a Facility made available to Artifacts in the context of an Organization."@en ;
    rdfs:label "proposes facility"@en, "fournit de facilité"@fr .

:hasOrganizationalValue a owl:ObjectProperty ;
    rdfs:isDefinedBy :regulation ;
    rdfs:domain :Organization ;
    rdfs:range :OrganizationalValue ;
    rdfs:comment "A relation that refers to an Organization Value of an Organization."@en ;
    rdfs:label "has organizational value"@en, "a une valeur organisationnelle"@fr .

:isMembershipOf a owl:ObjectProperty ;
    rdfs:isDefinedBy :regulation ;
    rdfs:domain :Membership ;
    rdfs:range :Agent ;
    rdfs:comment "A relation that refers to the Agent involved in a Membership."@en ;
    rdfs:label "is membership of"@en, "est l'appartenance à"@fr .

:isMembershipFor a owl:ObjectProperty ;
    rdfs:isDefinedBy :regulation ;
    rdfs:domain :Membership ;
    rdfs:range :Role ;
    rdfs:comment "A relation that refers to the Role involved in a Membership."@en ;
    rdfs:label "is membership for"@en, "est l'adhésion pour"@fr .

:isMembershipIn a owl:ObjectProperty ;
    rdfs:isDefinedBy :regulation ;
    rdfs:domain :Membership ;
    rdfs:range :Group ;
    rdfs:comment "A relation that refers to the Group involved in a Membership."@en ;
    rdfs:label "is membership in"@en, "est l'appartenance à"@fr .

:hasMembershipRelationshipWith a owl:ObjectProperty ;
    rdfs:isDefinedBy :regulation ;
    rdfs:domain :Membership ;
    rdfs:range :Membership ;
    rdfs:comment "A relation that refers to the relationship between Agents member of two Memberships."@en ;
    rdfs:label "has membership relationship with"@en, "a une relation d'affiliation avec"@fr .

:structures a owl:ObjectProperty ;
    rdfs:isDefinedBy :regulation ;
    rdfs:domain :Group ;
    rdfs:range :Organization ;
    rdfs:inverseOf :isStructuredBy ;
    rdfs:comment "A relation that refers to a Group that structures an Organization."@en ;
    rdfs:label "structures"@en, "structure"@fr .

:isStructuredBy a owl:ObjectProperty ;
    rdfs:isDefinedBy :regulation ;
    rdfs:domain :Organization ;
    rdfs:range :Group ;
    rdfs:inverseOf :structures ;
    rdfs:comment "A relation that refers to an Organization that is structured by a Group."@en ;
    rdfs:label "is structured by"@en, "est structuré par"@fr .

:isSubGroupOf a owl:ObjectProperty ;
    rdfs:isDefinedBy :regulation ;
    rdfs:domain :Group ;
    rdfs:range :Group ;
    rdfs:comment "A relation that refers to a subgroup relationship between two Groups."@en ;
    rdfs:label "is subgroup of"@en, "est un sous-groupe de"@fr .

:proposesProcess a owl:ObjectProperty ;
    rdfs:isDefinedBy :regulation ;
    rdfs:domain :Organization ;
    rdfs:range :Process ;
    rdfs:comment "A relation that refers to a Process that can be executed in the context of an Organization. "@en ;
    rdfs:label "proposes process"@en, "fournit un processus"@fr .

:includesMission a owl:ObjectProperty ;
    rdfs:isDefinedBy :regulation ;
    rdfs:domain :Process ;
    rdfs:range :Mission ;
    rdfs:comment "A relation that refers to a Mission part of a Process."@en ;
    rdfs:label "includes mission"@en, "inclut la mission"@fr .

:includesOrganizationalGoal a owl:ObjectProperty ;
    rdfs:isDefinedBy :regulation ;
    rdfs:domain :Mission ;
    rdfs:range :OrganizationalGoal ;
    rdfs:comment "A relation that refers to an Organizational Goal involved in a Mission."@en ;
    rdfs:label "includes organizational goal"@en, "inclut le but de l'organization"@fr .

:isDependentOnOrganizationalGoal a owl:ObjectProperty ;
    rdfs:isDefinedBy :regulation ;
    rdfs:domain :OrganizationalGoal ;
    rdfs:range :OrganizationalGoal ;
    rdfs:comment "A relation that refers to the way in which two Organizational Goals are related to each other, and one is affected by the other."@en ;
    rdfs:label "is dependent on organizational goal"@en, "dépend du but de l'organisation"@fr .
    
:isCommitmentFor a owl:ObjectProperty ;
    rdfs:isDefinedBy :regulation ;
    rdfs:domain :Commitment ;
    rdfs:range :Mission ;
    rdfs:comment "A relation that refers to a commitment for a Mission."@en ;
    rdfs:label "is commitment for"@en, "est engagement pour"@fr .

:isCommitmentOf a owl:ObjectProperty ;
    rdfs:isDefinedBy :regulation ;
    rdfs:domain :Commitment ;
    rdfs:range :Agent ;
    rdfs:comment "A relation that refers to a commitment of an Agent."@en ;
    rdfs:label "is commitment of"@en, "est engagement de"@fr .

:isAccessTo a owl:ObjectProperty ;
    rdfs:isDefinedBy :regulation ;
    rdfs:domain :Access ;
    rdfs:range :Artifact ;
    rdfs:comment "A relation that refers to an Artifact involved in an Access."@en ;
    rdfs:label "is access to"@en, "est l'accès à"@fr .

:isAccessOf a owl:ObjectProperty ;
    rdfs:isDefinedBy :regulation ;
    rdfs:domain :Access ;
    rdfs:range :Agent ;
    rdfs:comment "A relation that refers to an Agent involved in an Access."@en ;
    rdfs:label "is access of"@en, "est l'accès de"@fr .

:isAccessFor a owl:ObjectProperty ;
    rdfs:isDefinedBy :regulation ;
    rdfs:domain :Access ;
    rdfs:range :Usage ;
    rdfs:comment "A relation that refers to a Usage involved in an Access."@en ;
    rdfs:label "is access for"@en, "est l'accès pour"@fr .

:isUsageOf a owl:ObjectProperty ;
    rdfs:isDefinedBy :regulation ;
    rdfs:domain :Usage ;
    rdfs:range :Facility ;
    rdfs:comment "A relation that refers to a Facility involved in a Usage."@en ;
    rdfs:label "is usage of"@en, "est un usage de"@fr .

:isUsageIn a owl:ObjectProperty ;
    rdfs:isDefinedBy :regulation ;
    rdfs:domain :Usage ;
    rdfs:range :Setting ;
    rdfs:comment "A relation that refers to a Setting involved in a Usage."@en ;
    rdfs:label "is usage in"@en, "est un usage dans"@fr .

:hasUsageRelationshipWith a owl:ObjectProperty ;
    rdfs:isDefinedBy :regulation ;
    rdfs:domain :Usage ;
    rdfs:range :Usage ;
    rdfs:comment "A relation that refers to the relationship between two Usages."@en ;
    rdfs:label "has usage relationship with"@en, "a une relation d'usage avec"@fr .

:hasFacility a owl:ObjectProperty ;
    rdfs:isDefinedBy :regulation ;
    rdfs:domain :Artifact ;
    rdfs:range :Facility ;
    rdfs:comment "A relation that refers to a Facility of an Artifact."@en ;
    rdfs:label "has facility"@en, "a pour potentialité d'usage"@fr .

:isSettingOf a owl:ObjectProperty ;
    rdfs:isDefinedBy :regulation ;
    rdfs:domain :Setting ;
    rdfs:range :Organization ;
    rdfs:comment "A relation that refers to a Setting of an Organization."@en ;
    rdfs:label "is setting of"@en, "est un contexte d'usage de"@fr .

:proposesSetting a owl:ObjectProperty ;
    rdfs:isDefinedBy :regulation ;
    rdfs:domain :Organization ;
    rdfs:range :Setting ;
    rdfs:comment "A relation that refers to a Setting that can be used in the context of an Organization."@en ;
    rdfs:label "proposes setting"@en, "fournit un contexte d'usage"@fr .
