
@base <https://purl.org/hmas/> .
@prefix : <> .
@prefix hmas: <https://purl.org/hmas/core#> .

@prefix owl: <http://www.w3.org/2002/07/owl#> .
@prefix rdf: <http://www.w3.org/1999/02/22-rdf-syntax-ns#> .
@prefix xml: <http://www.w3.org/XML/1998/namespace> .
@prefix xsd: <http://www.w3.org/2001/XMLSchema#> .
@prefix rdfs: <http://www.w3.org/2000/01/rdf-schema#> .
@prefix cc: <http://creativecommons.org/ns#> .
@prefix vann: <http://purl.org/vocab/vann/> .
@prefix voaf: <http://purl.org/vocommons/voaf#> .
@prefix foaf: <http://xmlns.com/foaf/0.1/>.
@prefix schema: <http://schema.org/>.
@prefix dct: <http://purl.org/dc/terms/>.
@prefix skos: <http://www.w3.org/2004/02/skos/core#>.

#################################################################
#    Ontology Description
#################################################################

:regulation rdf:type owl:Ontology ;
    dct:title "Hypermedia MAS Regulation Ontology"@en, "Ontologie de Régulation des SMA Hypermédias"@fr ;
    dct:description "An ontology to describe the regulation of Hypermedia Multi-Agent Systems."@en,
    "L'ontologie pour décrire la régulation des systèmes multi-agents hypermédias."@fr ;
    dct:issued "2022-05-01"^^xsd:date ;
    ## dct:contributor <http://ns.inria.fr/fabien.gandon#me> ;
    cc:license <https://creativecommons.org/licenses/by/4.0/> ;
    owl:imports :core ;
    vann:preferredNamespacePrefix "hmas" ;
    vann:preferredNamespaceUri <> .


<https://inria.fr/>
  schema:name "Inria" ;
  schema:url <https://inria.fr/> .

<https://www.mines-stetienne.fr/>
  schema:name "MINES Saint-Étienne" ;
  schema:url <https://mines-stetienne.fr> .

<https://www.unisg.ch/en>
  schema:name "University of St.Gallen" ;
  schema:url <https://www.unisg.ch> .

<https://orcid.org/0000-0002-4506-2745> a schema:Person ;
  schema:name "Luis Gustavo Nardin" ;
  schema:email "luisgustavo.nardin@emse.fr" ;
  schema:url <http://gnardin.github.io/website/> ;
  schema:identifier <https://orcid.org/0000-0002-4506-2745> ;
  schema:affiliation <https://www.mines-stetienne.fr/> .

<https://orcid.org/0000-0003-0821-6095> a schema:Person ;
  schema:name "Chistopher Leturc" ;
  schema:email "christopher.leturc@inria.fr" ;
  schema:url <https://www.linkedin.com/in/christopher-leturc/> ;
  schema:identifier <https://orcid.org/0000-0003-0821-6095> ;
  schema:affiliation <https://inria.fr/> .

#################################################################
#    Classes
#################################################################
:RegulativeNorm rdf:type owl:Class ;
    rdfs:isDefinedBy :regulation ;
    rdfs:comment "A specification of the standard behaviors one expects from others in an organization."@en ;
    rdfs:label "Norm"@en .

:PossibleWorld rdf:type owl:Class ;
    rdfs:isDefinedBy :regulation ;
    rdfs:comment "A possible world is a ressource that describes a state of affair of the world."@en ;
    rdfs:label "Normative Context"@en .

:NormativeContext rdf:subClassOf :PossibleWorld ;
    rdfs:isDefinedBy :regulation ;
    rdfs:comment "A context in which a norm is applicable."@en ;
    rdfs:label "Normative Context"@en .

:Obligation rdf:subClassOf :PossibleWorld ;
    rdfs:isDefinedBy :regulation ;
    rdfs:comment "A possible world that describes an obligation."@en ;
    rdfs:label "Obligation"@en .

:Permission rdf:subClassOf :PossibleWorld ;
    rdfs:isDefinedBy :regulation ;
    rdfs:comment "A possible world that describes a permission."@en ;
    rdfs:label "Permission"@en .

:Prohibition rdf:subClassOf :PossibleWorld ;
    rdfs:isDefinedBy :regulation ;
    rdfs:comment "A possible world that describes a prohibition."@en ;
    rdfs:label "Prohibition"@en .


:WebOfAgents rdf:type owl:Class ;
  rdfs:comment "Web of Agents is a subset of the web." ;
  rdsf:label "WebOfAgents"@en .

:RegulatedWeb rdf:type owl:Class ;
  rdfs:comment "A Regulated Web is a subset of the Web of Agents arranged in one or several Situated Regulated Organization Enttities."@en ;
  rdfs:label "RegulatedWeb"@en .

:SituatedRegulatedOrganizationEntity rdf:type owl:Class ;
  rdfs:comment "An organization entity situated on agents and artifacts, and regulated by a normative system."@en ;
  rdfs:label "SituatedRegulatedOrganizationEntity"@en .

:InstitutionEntity rdf:type owl:Class ;
  rdfs:comment "An Institution entity situates artifacts (events, states) and agents (actions) in the regulations and organization of Situated Regulated Organization Entities."@en ;
  rdfs:label "InstitutionEntity"@en .

:TestRegulation a owl:Class ;
  rdfs:comment "testing the redirections"@en ;
  rdfs:isDefinedBy :regulation .


:AuthorityRole rdf:subClassOf hmas:SocialRole ;
    rdfs:isDefinedBy :regulation ;
    rdfs:comment "The authority who has a power to apply a norm and which is in charge of applying the norm. It may be an :Agent or an :Organization. "@en ;
    rdfs:label "Authority"@en .

#################################################################
#    Object Properties
#################################################################

:enforcesRegulativeNorm rdf:type owl:ObjectProperty ;
    rdfs:isDefinedBy :regulation ;
    rdfs:domain :Organization ;
    rdfs:range :RegulativeNorm ;
    rdfs:comment "An organization enforces a norm. "@en ;
    rdfs:label "enforces the norm"@en .

:definesRegulativeNorm rdf:type owl:ObjectProperty ;
    rdfs:isDefinedBy :regulation ;
    rdfs:domain :Organization ;
    rdfs:range :RegulativeNorm ;
    rdfs:comment "An organization Specification defines a norm. "@en ;
    rdfs:label "defines the norm"@en .

:hasNormativeTarget rdf:type owl:ObjectProperty ;
    rdfs:isDefinedBy :regulation ;
    rdfs:domain :RegulativeNorm ;
    rdfs:range :Role ;
    rdfs:comment "An agent or a group of agents concerned by a norm." ;
    rdfs:label "has normative target".

:beInChargeOfEnforcingTheRegulativeNorm rdf:type owl:ObjectProperty ;
    rdfs:isDefinedBy :regulation ;
    rdfs:domain :RegulativeNorm ;
    rdfs:range :AuthorityRole;
    rdfs:comment "It defines who is the authority in charge of applying the norm. "@en ;
    rdfs:label "be in charge of enforcing the regulative norm"@en .


:isPossiblyDescribedBy rdf:type owl:ObjectProperty ;
    rdfs:isDefinedBy :regulation ;
    rdfs:domain :Workspace ;
    rdfs:range :PossibleWorld ;
    rdfs:comment "A workspace state is associated with a set of possible worlds. "@en ;
    rdfs:label "has a possible world"@en .

:hasDeonticSpecification rdf:type owl:ObjectProperty ;
    rdfs:isDefinedBy :regulation ;
    rdfs:domain :PossibleWorld ;
    rdfs:range :RegulativeNorm ;
    rdfs:comment "A possible world may have some deontic specifications. "@en ;
    rdfs:label "has deontic specification"@en .

:prohibits rdf:type owl:ObjectProperty ;
    rdfs:isDefinedBy :regulation ;
    rdfs:domain :RegulativeNorm ;
    rdfs:range :Prohibition ;
    rdfs:comment "A prohibition is associated with a norm and describes a state of affairs that shouldn't be verified when a norm is applied. "@en ;
    rdfs:label "prohibits"@en .

:permits rdf:type owl:ObjectProperty ;
    rdfs:isDefinedBy :regulation ;
    rdfs:domains :RegulativeNorm ;
    rdfs:range :Permission ;
    rdfs:comment "A permission is associated with a norm and describes a state of affairs which is explicitly permitted when a norm is applied."@en ;
    rdfs:label "allows"@en .

:obliges rdf:type owl:ObjectProperty ;
    rdfs:isDefinedBy :regulation ;
    rdfs:domain :RegulativeNorm ;
    rdfs:range :Obligation ;
    rdfs:comment "An obligation is associated with a norm and describes a state of affairs that must be maintained when a norm is applied."@en ;
    rdfs:label "obliges"@en .

:hasDeonticSpecification rdf:type owl:ObjectProperty ;
    rdfs:isDefinedBy :regulation ;
    rdfs:domain :PossibleWorld ;
    rdfs:range :RegulativeNorm ;
    rdfs:comment "A possible world may have some deontic specifications. "@en ;
    rdfs:label "has deontic specification"@en .

:hasNormativeContext rdf:type owl:ObjectProperty ;
    rdfs:isDefinedBy :regulation ;
    rdfs:domain :RegulativeNorm ;
    rdfs:range :NormativeContext ;
    rdfs:comment "A specification which defines when a norm is applicable. "@en ;
    rdfs:label "has normative context"@en .

:includes a owl:ObjectProperty ;
            rdfs:domain :SituatedRegulatedOrganizationEntity ;
            rdfs:range :SituatedRegulatedOrganizationEntity ;
            rdfs:comment "A relation of containment of two Situation Regulated Organization Entities."@en ;
            rdfs:label "includes"@en .

# Are the Workspace or the Agents and Artifacts that situate a SROE?
:situates a owl:ObjectProperty ;
            owl:inverseOf :isSituatedIn ;
            rdfs:domain [
              core:Agent ;
              core:Artifact
            ] ;
            rdfs:range :SituatedRegulatedOrganizationEntity ;
            rdfs:comment "A relation that specifies that agents and artifacts are part and regulated by the Situated Regulated Organization Entity."@en ;
            rdfs:label "situates"@en .

:isSituatedIn a owl:ObjectProperty ;
                owl:inverseOf :situates ;
                rdfs:domain :SituatedRegulatedOrganizationEntity ;
                rdfs:range [
                  core:Agent ;
                  core:Artifact
                ] ;
                rdfs:comment "A relation that specifies that a Situated Regulated Organization Entity includes and regulates a set of agents and artifacts."@en ;
                rdfs:label "is situated in"@en .

# Unsure about the domain and range because we may not be dealing only with single resources, but with set of resources
# Will we require regulations to be defined w.r.t. institutional facts only? If so, everything will have to be constituted as an Institutional Fact before they can be regulated.
:countAs a owl:ObjectProperty ;
           rdfs:domain rdfs:Resource ;
           rdfs:range rdfs:Resource ;
           rdfs:comment "Links resources to institutional facts."@en ;
           rdfs:label "count-as"@en .


